spectec/test-rocq/theories/type_preservation.v
@@ -1,4 +1,3 @@
-(* Proof Start *)
 
 From Stdlib Require Import String List Unicode.Utf8 NArith Arith.
 From RecordUpdate Require Import RecordSet.
@@ -10,18 +9,30 @@ Import RecordSetNotations.
 From WasmSpectec Require Import wasm helper_lemmas helper_tactics typing_lemmas.
 From mathcomp Require Import ssreflect ssrfun ssrnat ssrbool seq.
 
-(* Theorems *)
+Lemma inst_t_context_local_empty: forall s i C,
+	Module_instance_ok s i C ->
+    C_LOCALS C = [].
+Proof.
+	move => s i C HMInst. inversion HMInst => //=.
+Qed.
 
-Theorem t_pure_preservation: forall v_S v_C  v_func_type,
+Lemma inst_t_context_labels_empty: forall s i C,
+	Module_instance_ok s i C ->
+    C_LABELS C = [].
+Proof.
+	move => s i C HMInst. inversion HMInst => //=.
+Qed.
+
+		
+Lemma Step_pure__unreachable_preserves : forall v_S v_C  v_func_type,
 	Admin_instrs_ok v_S v_C [(AI_UNREACHABLE )] v_func_type ->
 	Step_pure [(AI_UNREACHABLE )] [(AI_TRAP )] ->
 	Admin_instrs_ok v_S v_C [(AI_TRAP )] v_func_type.
 Proof.
-	move=> v_S v_C v_func_type HType HReduce.
-	destruct v_func_type as [v_t_1 v_t_2].
-	apply (AIs_ok_seq v_S v_C [] (AI_TRAP) v_t_1 v_t_2 v_t_1).
-    - apply admin_weakening_empty_both.
-	    apply AIs_ok_empty.
+	move => v_S v_C v_func_type HType HReduce.
+	destruct v_func_type as [tf1 tf2].
+	apply (AIs_ok_seq v_S v_C [] (AI_TRAP) tf1 tf2 tf1).
+	- apply admin_weakening_empty_both. apply AIs_ok_empty.
 	- apply AI_ok_trap.
 Qed.
 
@@ -32,31 +43,2352 @@ Lemma Step_pure__nop_preserves : forall v_S v_C  v_func_type,
 Proof.
 	move => v_S v_C v_func_type HType HReduce.
 	destruct v_func_type as [tf1 tf2].
-
-	let ts1 := fresh "ts1_comp" in
-    let ts2 := fresh "ts2_comp" in
-    let ts3 := fresh "ts3_comp" in
-    let ts4 := fresh "ts4_comp" in
-    let H1 := fresh "H1_comp" in
-    let H2 := fresh "H2_comp" in
-    let H3 := fresh "H3_comp" in
-    let H4 := fresh "H4_comp" in
-	rewrite -> app_left_single_nil in HType;
-    apply admin_composition_typing_single in HType; destruct HType as [ts1 [ts2 [ts3 [ts4 [H1 [H2 [H3 H4]]]]]]];
-	try apply admin_empty in H3.
-	
-	subst.
-	apply Admin_instrs_ok__frame.
+	apply_composition_typing_single HType; subst.
+	apply AIs_ok_frame.
 	apply Nop_typing in H4_comp; subst.
 	apply admin_weakening_empty_both.
-	apply Admin_instrs_ok__empty.
+	apply AIs_ok_empty.
+Qed.
+
+Lemma Step_pure__drop_preserves : forall v_S v_C (v_val : val) v_func_type,
+	Admin_instrs_ok v_S v_C [(v_val : admininstr);(AI_DROP )] v_func_type ->
+	Step_pure [(v_val : admininstr);(AI_DROP )] [] ->
+	Admin_instrs_ok v_S v_C [] v_func_type.
+Proof.
+	move => v_S v_C v_val v_func_type HType HReduce.
+	destruct v_func_type as [tf1 tf2].
+	apply_composition_typing_and_single HType.
+	apply_composition_typing_single H4_comp.
+
+	apply Drop_typing in H4_comp1; destruct H4_comp1 as [t H1]; subst.
+	apply_const_typing_to_val H4_comp0.
+	subst.
+	repeat rewrite -> app_assoc in H1_comp1; apply split_append_last in H1_comp1; destruct H1_comp1; subst.
+	rewrite H.
+	apply admin_weakening_empty_both.
+	apply AIs_ok_empty.
+Qed.
+
+Lemma Step_pure__select_true_preserves : forall v_S v_C (v_val_1 : val) (v_val_2 : val) (v_c : iN 32) v_func_type,
+	Admin_instrs_ok v_S v_C [(v_val_1 : admininstr);(v_val_2 : admininstr);(AI_CONST I32 (v_c));(AI_SELECT )] v_func_type ->
+	Step_pure [(v_val_1 : admininstr);(v_val_2 : admininstr);(AI_CONST I32 (v_c));(AI_SELECT )] [(v_val_1 : admininstr)] ->
+	Admin_instrs_ok v_S v_C [(v_val_1 : admininstr)] v_func_type.
+Proof.
+	move => v_S v_C v_val_1 v_val_2 v_c v_func_type HType HReduce.
+	destruct v_func_type as [tf1 tf2].
+	apply_composition_typing_and_single HType.
+	apply_composition_typing_and_single H4_comp.
+	apply_composition_typing_and_single H4_comp1.
+	apply_composition_typing_single H4_comp2.
+	induction v_val_1.
+	apply AI_const_typing in H4_comp0.
+	apply_const_typing_to_val H4_comp.
+	apply AI_const_typing in H4_comp1.
+	apply Select_typing in H4_comp3; destruct H4_comp3 as [v_ts [v_t [H4_comp3 H4_comp3']]].
+	subst.
+	remember [:: v_t; v_t; I32] as v_select.
+	rewrite -cat1s in Heqv_select.
+	remember [:: v_t; I32] as v_select2.
+	rewrite -cat1s in Heqv_select2; subst.
+	repeat rewrite -> app_assoc in H1_comp2.
+	apply split_append_last in H1_comp2; destruct H1_comp2.
+	rewrite H in H1_comp0.
+	repeat rewrite -> app_assoc in H1_comp0.
+	apply split_append_last in H1_comp0; destruct H1_comp0.
+	rewrite H1 in H1_comp1.
+	repeat rewrite -> app_assoc in H1_comp1.
+	apply split_append_last in H1_comp1; destruct H1_comp1.
+	rewrite H3.
+	repeat rewrite -> app_assoc.
+	apply admin_instrs_weakening_empty_1.
+	apply (AIs_ok_seq v_S v_C [] (VAL_CONST v_valtype v_val_) [] [v_t] []). 
+	apply AIs_ok_empty.
+	unfold fun_coec_val__admininstr.
+	apply (AI_ok_instr v_S v_C (CONST v_valtype v_val_) (mk_functype [] [v_t])); subst.
+	apply const.
+Qed.
+
+Lemma Step_pure__select_false_preserves : forall v_S v_C (v_val_1 : val) (v_val_2 : val) (v_c : iN 32) v_func_type,
+	Admin_instrs_ok v_S v_C [(v_val_1 : admininstr);(v_val_2 : admininstr);(AI_CONST I32 v_c);(AI_SELECT )] v_func_type ->
+	Step_pure [(v_val_1 : admininstr);(v_val_2 : admininstr);(AI_CONST I32 v_c);(AI_SELECT )] [(v_val_2 : admininstr)] ->
+	Admin_instrs_ok v_S v_C [(v_val_2 : admininstr)] v_func_type.
+Proof.
+	move => v_S v_C v_val_1 v_val_2 v_c v_func_type HType HReduce.
+	destruct v_func_type as [tf1 tf2].
+	apply_composition_typing_and_single HType.
+	apply_composition_typing_and_single H4_comp.
+	apply_composition_typing_and_single H4_comp1.
+	apply_composition_typing_single H4_comp2.
+	apply_const_typing_to_val H4_comp0.
+	induction v_val_2.
+	apply AI_const_typing in H4_comp.
+	apply AI_const_typing in H4_comp1.
+	apply Select_typing in H4_comp3; destruct H4_comp3 as [v_ts [v_t [H4_comp3 H4_comp3']]].
+	subst.
+	remember [:: v_t; v_t; I32] as v_select.
+	rewrite -cat1s in Heqv_select.
+	remember [:: v_t; I32] as v_select2.
+	rewrite -cat1s in Heqv_select2; subst.
+	repeat rewrite -> app_assoc in H1_comp2.
+	apply split_append_last in H1_comp2; destruct H1_comp2.
+	rewrite H in H1_comp0.
+	repeat rewrite -> app_assoc in H1_comp0.
+	apply split_append_last in H1_comp0; destruct H1_comp0.
+	rewrite H1 in H1_comp1.
+	repeat rewrite -> app_assoc in H1_comp1.
+	apply split_append_last in H1_comp1; destruct H1_comp1.
+	rewrite H3.
+	repeat rewrite -> app_assoc.
+	apply admin_instrs_weakening_empty_1.
+	apply (AIs_ok_seq v_S v_C [] (VAL_CONST v_valtype0 v_val_0) [] [v_t] []). 
+	apply AIs_ok_empty.
+	unfold fun_coec_val__admininstr.
+	apply (AI_ok_instr v_S v_C (CONST v_valtype0 v_val_0) (mk_functype [] [v_t])); subst.
+	apply const.
+Qed.
+
+Lemma Step_pure__if_true_preserves : forall v_S v_C (v_c : iN 32) (v_t : (option valtype)) (v_instr_1 : (list instr)) (v_instr_2 : (list instr)) v_func_type,
+	Admin_instrs_ok v_S v_C [(AI_CONST I32 v_c);(AI_IFELSE v_t v_instr_1 v_instr_2)] v_func_type ->
+	Step_pure [(AI_CONST I32 v_c);(AI_IFELSE v_t v_instr_1 v_instr_2)] [(AI_BLOCK v_t v_instr_1)] ->
+	Admin_instrs_ok v_S v_C [(AI_BLOCK v_t v_instr_1)] v_func_type.
+Proof.
+	move => v_S v_C v_c v_t v_instr_1 v_instr_2 v_func_type HType HReduce.
+	destruct v_func_type as [ts1 ts2].
+	apply_composition_typing_and_single HType.
+	apply_composition_typing_single H4_comp.
+	apply AI_const_typing in H4_comp0.
+	apply If_typing in H4_comp1; destruct H4_comp1 as [ts0 [H1 [H2 [H3 H4]]]].
+	subst.
+	repeat rewrite -> app_assoc in H1_comp1.
+	apply split_append_last in H1_comp1; destruct H1_comp1.
+	rewrite H.
+	repeat rewrite -> app_assoc.
+	apply admin_instrs_weakening_empty_1.
+	apply (AIs_ok_seq v_S v_C [] (AI_BLOCK v_t v_instr_1) [] v_t []). 
+	apply AIs_ok_empty.
+	apply (AI_ok_instr v_S v_C (BLOCK v_t v_instr_1) (mk_functype [::] v_t)).
+	apply (block).
+	rewrite <- upd_label_is_same_as_append.
+	apply H3.
+Qed.
+
+Lemma Step_pure__if_false_preserves : forall v_S v_C (v_c : iN 32) (v_t : (option valtype)) (v_instr_1 : (list instr)) (v_instr_2 : (list instr)) v_func_type,
+	Admin_instrs_ok v_S v_C [(AI_CONST I32 v_c);(AI_IFELSE v_t v_instr_1 v_instr_2)] v_func_type ->
+	Step_pure [(AI_CONST I32 v_c);(AI_IFELSE v_t v_instr_1 v_instr_2)] [(AI_BLOCK v_t v_instr_2)] ->
+	Admin_instrs_ok v_S v_C [(AI_BLOCK v_t v_instr_2)] v_func_type.
+Proof.
+	move => v_S v_C v_c v_t v_instr_1 v_instr_2 v_func_type HType HReduce.
+	destruct v_func_type as [ts1 ts2].
+	apply_composition_typing_and_single HType.
+	apply_composition_typing_single H4_comp.
+	apply AI_const_typing in H4_comp0.
+	apply If_typing in H4_comp1; destruct H4_comp1 as [H1 [H2 [H3 H4]]].
+	subst.
+	repeat rewrite -> app_assoc in H1_comp1.
+	apply split_append_last in H1_comp1; destruct H1_comp1.
+	rewrite H.
+	repeat rewrite -> app_assoc.
+	apply admin_instrs_weakening_empty_1.
+	apply (AIs_ok_seq v_S v_C [] (AI_BLOCK v_t v_instr_2) [] v_t []). 
+	apply AIs_ok_empty.
+	apply (AI_ok_instr v_S v_C (BLOCK v_t v_instr_2) (mk_functype [::] v_t)).
+	apply block.
+	rewrite <- upd_label_is_same_as_append.
+	apply H4.
+Qed.
+
+Lemma Step_pure__label_vals_preserves : forall v_S v_C (v_n : n) (v_instr : (list instr)) (v_val : (list val)) v_func_type,
+	Admin_instrs_ok v_S v_C [(AI_LABEL_ v_n v_instr (map fun_coec_val__admininstr v_val))] v_func_type ->
+	Step_pure [(AI_LABEL_ v_n v_instr (map fun_coec_val__admininstr v_val))] (map fun_coec_val__admininstr v_val) ->
+	Admin_instrs_ok v_S v_C (map fun_coec_val__admininstr v_val) v_func_type.
+Proof.
+	move => v_S v_C v_n v_instr v_val v_func_type HType HReduce.
+	destruct v_func_type as [ts1 ts2].
+	apply_composition_typing_single HType.
+	apply Label_typing in H4_comp; destruct H4_comp as [ts [ts2' [H1 [H2 [H3 H4]]]]].
+	subst.
+	repeat rewrite -> app_assoc.
+	apply admin_instrs_weakening_empty_1.
+	apply Val_Const_list_typing in H4; subst.
+	rewrite H4.
+	simpl.
+	apply Const_list_typing_empty.
+Qed.
+
+Lemma Step_pure__br_zero_preserves : forall v_S v_C (v_n : n) (v_instr' : (list instr)) (v_val' : (list val)) (v_val : (list val)) (v_instr : (list instr)) v_func_type,
+	Admin_instrs_ok v_S v_C [(AI_LABEL_ v_n v_instr' (@app _ (map fun_coec_val__admininstr v_val') (@app _ (map fun_coec_val__admininstr v_val) (@app _ [AI_BR 0] (map fun_coec_instr__admininstr v_instr)))))] v_func_type ->
+	((List.length v_val) = v_n) ->
+	Admin_instrs_ok v_S v_C (@app _ (map fun_coec_val__admininstr v_val) (map fun_coec_instr__admininstr v_instr')) v_func_type.
+Proof.
+	move => v_S v_C v_n v_instr' v_val' v_val v_instr v_func_type HType HLength.
+	destruct v_func_type as [ts1 ts2].
+	rewrite <- admin_instrs_ok_eq in HType.
+	apply Label_typing in HType; destruct HType as [ts [ts2' [? [? [? ?]]]]].
+	apply_composition_typing H2.
+	apply_composition_typing H4_comp.
+	apply_composition_typing H4_comp0.
+	repeat rewrite <- app_right_nil in *.
+	rewrite <- admin_instrs_ok_eq in H3_comp1.
+	apply Break_typing in H3_comp1; destruct H3_comp1 as [ts0' [ts1' [? [? ?]]]].
+	apply Val_Const_list_typing in H3_comp.
+	apply Val_Const_list_typing in H3_comp0.
+	apply empty_append in H1_comp; destruct H1_comp.
+	subst. simpl in *.
+	unfold upd_label, lookup_total in H1_comp1.
+	simpl in H1_comp1.
+	apply admin_instrs_weakening_empty_1.
+	apply admin_composition' with (t2s := ts).
+	repeat rewrite -> app_assoc in H1_comp1.
+	eapply concat_cancel_last_n in H1_comp1; destruct H1_comp1; subst.
+	rewrite <- H2.
+	apply Const_list_typing_empty.
+	rewrite List.map_length.
+	destruct ts => //=. 
+	eapply AIs_ok_instrs in H0; eauto.
 Qed.
 
 
+Lemma Step_pure__br_succ_preserves : forall v_S v_C (v_n : n) (v_instr' : (list instr)) (v_val : (list val)) (v_l : labelidx) (v_instr : (list instr)) v_func_type,
+	Admin_instrs_ok v_S v_C [(AI_LABEL_ v_n v_instr' (@app _ (map fun_coec_val__admininstr v_val) (@app _ [AI_BR (v_l + 1)] (map fun_coec_instr__admininstr v_instr))))] v_func_type ->
+	Step_pure [(AI_LABEL_ v_n v_instr' (@app _ (map fun_coec_val__admininstr v_val) (@app _ [AI_BR (v_l + 1)] (map fun_coec_instr__admininstr v_instr))))] (@app _ (map fun_coec_val__admininstr v_val) [(AI_BR v_l)]) ->
+	Admin_instrs_ok v_S v_C (@app _ (map fun_coec_val__admininstr v_val) [(AI_BR v_l)]) v_func_type.
+Proof.
+	move => v_S v_C v_n v_instr' v_val v_l v_instr v_func_type HType HReduce.
+	destruct v_func_type as [ts1 ts2].
+	rewrite <- admin_instrs_ok_eq in HType.
+	apply Label_typing in HType; destruct HType as [ts [ts2' [? [? [? ?]]]]].
+	apply_composition_typing H2.
+	apply_composition_typing H4_comp.
+	rewrite <- admin_instrs_ok_eq in H3_comp0.
+	repeat rewrite <- app_right_nil in *.
+	apply Val_Const_list_typing in H3_comp.
+	apply Break_typing in H3_comp0. destruct H3_comp0 as [ts0 [ts1' [? [? ?]]]].
+	subst.
+	apply empty_append in H1_comp; destruct H1_comp; subst.
+	simpl in *.
+	apply admin_instrs_weakening_empty_1.
+	eapply admin_composition'.
+	apply Const_list_typing_empty.
+	rewrite H1_comp0.
+	rewrite H2_comp.
+	apply AIs_ok_frame.
+	rewrite <- admin_instrs_ok_eq.
+	apply AI_ok_instr with (v_instr := BR v_l).
+	apply br.
+	- rewrite addn1 in H.
+	  unfold lt in H.
+	  move: H => /leP Hbool. auto.
+	- unfold lookup_total. by rewrite addn1.
+Qed.
+
+Lemma Step_pure__preserves__br_if_true : 
+  forall (v_l : labelidx) (v_c : iN 32) (v_ft : functype) (v_C : context) (v_s : store), 
+  ((Admin_instrs_ok v_s v_C [(AI_CONST I32 v_c);(AI_BR_IF v_l)] v_ft) -> 
+  ((Step_pure [(AI_CONST I32 v_c);(AI_BR_IF v_l)] [(AI_BR v_l)]) -> 
+  ((v_c <> mk_uN 32 0) -> 
+  (Admin_instrs_ok v_s v_C [(AI_BR v_l)] v_ft)))).
+Proof.
+  move => l c ft C s Hadmin Hstep Hval.
+  destruct ft as [ts1 ts2].
+	apply_composition_typing_and_single Hadmin.
+	apply_composition_typing_single H4_comp.
+  destruct l.
+  apply Br_if_typing in H4_comp1; destruct H4_comp1 as [ts [ts' [H1 [H2 [H3 H4]]]]].
+  apply AI_const_typing in H4_comp0.
+  subst.
+  repeat rewrite -> app_assoc in H1_comp1; apply split_append_last in H1_comp1; destruct H1_comp1.
+  rewrite H.
+  repeat rewrite -> app_assoc.
+  apply AIs_ok_frame.
+  remember (lookup_total (C_LABELS C) v_i) as ts'.
+  apply (AIs_ok_seq s C [] (AI_BR v_i) ts' ts' ts').
+  apply admin_weakening_empty_both. apply AIs_ok_empty.
+  apply (AI_ok_instr _ _ (BR v_i) (mk_functype ts' ts')).
+  apply (br C (v_i) [] ts' ts') => //=.
+  move: H3 => /leP Hbool. auto. 
+Qed.
+
+(* TODO: Example of migrating proofs using auto-translated statements (SSReflect) *)
+Lemma cat_app : 
+  forall {A : Type} (s1 s2 : seq A),
+  app s1 s2 = cat s1 s2.
+Proof. by []. Qed.
+
+Lemma cat_inv : 
+  forall {A : Type} (s1 : seq A) (s2 : seq A) (x1 : A) (x2 : A),
+	s1 ++ [:: x1] = s2 ++ [::x2] ->
+	s1 = s2 /\ x1 = x2.
+Proof. by apply: app_inj_tail. Qed.
+
+Lemma Admin_instrs_ok_admin_instr_ok : forall s C e ts1 ts2,
+  Admin_instrs_ok s C [:: e] (mk_functype ts1 ts2) ->
+  exists ts ts1' ts2', 
+    ts1 = ts ++ ts1' /\
+    ts2 = ts ++ ts2' /\
+    Admin_instr_ok s C e (mk_functype ts1' ts2').
+Proof.
+  move=> s C e ts1 ts2 Hadmin.
+  rewrite -[[:: _]]cat0s -cat_app in Hadmin.
+  move/admin_composition_typing_single: Hadmin => [ts [ts1' [ts2' [ts3 [Hts1 [Hts2 [Hempty Hadmin]]]]]]].
+  exists ts, ts1', ts2'; do ? split.
+  - by rewrite -cat_app.
+  - by rewrite -cat_app.
+  - move/admin_empty_same_type: Hempty => Hts3. 
+    by rewrite -{}Hts3 in Hadmin.
+Qed.
+
+Lemma Step_pure__br_if_true_preserves : forall v_S v_C (v_c : iN 32) (v_l : labelidx) v_func_type,
+	Admin_instrs_ok v_S v_C [(AI_CONST I32 v_c);(AI_BR_IF v_l)] v_func_type ->
+	Step_pure [(AI_CONST I32 v_c);(AI_BR_IF v_l)] [(AI_BR v_l)] ->
+	Admin_instrs_ok v_S v_C [(AI_BR v_l)] v_func_type.
+Proof.
+	move => v_S v_C v_c v_l v_func_type HType HReduce.
+	destruct v_func_type as [ts1 ts2].
+	apply_composition_typing_and_single HType.
+	apply_composition_typing_single H4_comp.
+	destruct v_l.
+	apply Br_if_typing in H4_comp1; destruct H4_comp1 as [ts [ts' [H1 [H2 [H3 H4]]]]].
+	apply AI_const_typing in H4_comp0.
+	subst.
+	repeat rewrite -> app_assoc in H1_comp1; apply split_append_last in H1_comp1; destruct H1_comp1.
+	rewrite H.
+	repeat rewrite -> app_assoc.
+	apply AIs_ok_frame.
+	remember (lookup_total (C_LABELS v_C) v_i) as ts'.
+	apply (AIs_ok_seq v_S v_C [] (AI_BR v_i) ts' ts' ts').
+	apply admin_weakening_empty_both. apply AIs_ok_empty.
+	apply (AI_ok_instr _ _ (BR v_i) (mk_functype ts' ts')).
+	apply (br v_C v_i [] ts' ts').
+	move: H3 => /leP Hbool. auto.
+	subst. reflexivity.
+Qed.
+
+Lemma Step_pure__br_if_false_preserves : forall v_S v_C (v_c : iN 32) (v_l : labelidx) v_func_type,
+	Admin_instrs_ok v_S v_C [(AI_CONST I32 v_c);(AI_BR_IF v_l)] v_func_type ->
+	Step_pure [(AI_CONST I32 v_c);(AI_BR_IF v_l)] [] ->
+	Admin_instrs_ok v_S v_C [] v_func_type.
+Proof.
+	move => v_S v_C v_c v_l v_func_type HType HReduce.
+	destruct v_func_type as [ts1 ts2].
+	apply_composition_typing_and_single HType.
+	apply_composition_typing_single H4_comp.
+	destruct v_l.
+	apply Br_if_typing in H4_comp1; destruct H4_comp1 as [ts [ts' [H1 [H2 [H3 H4]]]]].
+	apply AI_const_typing in H4_comp0.
+	subst.
+	repeat rewrite -> app_assoc in H1_comp1; apply split_append_last in H1_comp1; destruct H1_comp1.
+	rewrite H.
+	repeat rewrite -> app_assoc.
+	apply admin_weakening_empty_both. apply AIs_ok_empty.
+Qed.
+
+Lemma Step_pure__br_table_lt_preserves : forall v_S v_C (v_i : nat) (v_l : (list labelidx)) (v_l' : labelidx) v_func_type,
+	Admin_instrs_ok v_S v_C [(AI_CONST I32 (v_i : u32));(AI_BR_TABLE v_l v_l')] v_func_type ->
+	Step_pure [(AI_CONST I32 (v_i : u32));(AI_BR_TABLE v_l v_l')] [(AI_BR (lookup_total v_l v_i))] ->
+	(v_i < Datatypes.length v_l) -> 
+	Admin_instrs_ok v_S v_C [(AI_BR (lookup_total v_l v_i))] v_func_type.
+Proof.
+	move => v_S v_C v_i v_l v_l' v_func_type HType HReduce H.
+	destruct v_func_type as [ts1 ts2].
+	apply_composition_typing_and_single HType.
+	apply_composition_typing_single H4_comp.
+	apply Br_table_typing in H4_comp1.
+	destruct H4_comp1 as [ts1' [ts [H1 [H2 [H3 [H4 H5]]]]]].
+	apply AI_const_typing in H4_comp0.
+	subst.
+	repeat rewrite -> app_assoc in H1_comp1.
+	apply split_append_last in H1_comp1; destruct H1_comp1.
+	rewrite H0.
+	repeat rewrite <- app_assoc.
+	apply AIs_ok_frame.
+	apply AIs_ok_frame.
+	remember (ts1' ++ lookup_total (C_LABELS v_C) v_l')%list as ts. (* Just for convencience *)
+	apply (AIs_ok_seq v_S v_C [] (AI_BR (lookup_total v_l v_i)) ts ts3_comp1 ts).
+	+ (* Empty *) apply admin_weakening_empty_both. apply AIs_ok_empty.
+	+ (* BR *) apply (AI_ok_instr _ _ (BR (lookup_total v_l v_i)) (mk_functype ts ts3_comp1)).
+		subst. apply (br v_C (lookup_total v_l v_i) ts1' (lookup_total (C_LABELS v_C) v_l') ts3_comp1).
+		rewrite Forall_nth in H5.
+		rewrite Forall_nth in H2.
+	  	move: H => /leP H.
+		apply (H5 _ default_val) in H as H6.
+		apply (H2 _ default_val) in H as H7.
+
+	  	move: H7 => /leP Hbool. auto.
+		rewrite -> Forall_forall in H5.
+		assert (In (lookup_total v_l v_i) v_l) as H4.
+		{ induction v_l as [| a l].
+		  - inversion H; subst.
+		  - move: H => /leP H.
+		    eapply nth_In in H.
+			unfold lookup_total.
+			apply H.
+		}
+		eapply H5 in H4. auto.
+Qed.
+
+Lemma Step_pure__br_table_ge_preserves : forall v_S v_C (v_i : nat) (v_l : (list labelidx)) (v_l' : labelidx) v_func_type,
+	Admin_instrs_ok v_S v_C [(AI_CONST I32 (v_i : u32));(AI_BR_TABLE v_l v_l')] v_func_type ->
+	Step_pure [(AI_CONST I32 (v_i : u32));(AI_BR_TABLE v_l v_l')] [(AI_BR v_l')] ->
+	(v_i >= (List.length v_l))%coq_nat ->
+	Admin_instrs_ok v_S v_C [(AI_BR v_l')] v_func_type.
+Proof.
+	move => v_S v_C v_i v_l v_l' v_func_type HType HReduce H.
+	destruct v_func_type as [ts1 ts2].
+	apply_composition_typing_and_single HType.
+	apply_composition_typing_single H4_comp.
+	apply Br_table_typing in H4_comp1; destruct H4_comp1 as [ts1' [ts [H1 [H2 [H3 [H4 H5]]]]]].
+	apply AI_const_typing in H4_comp0.
+	subst.
+	repeat rewrite -> app_assoc in H1_comp1.
+	apply split_append_last in H1_comp1; destruct H1_comp1.
+	rewrite H0.
+	repeat rewrite <- app_assoc.
+	apply AIs_ok_frame.
+	apply AIs_ok_frame.
+	remember (ts1' ++ lookup_total (C_LABELS v_C) v_l')%list as ts. (* Just for convencience *)
+	apply (AIs_ok_seq v_S v_C [] (AI_BR v_l') ts ts3_comp1 ts).
+	+ (* Empty *) apply admin_weakening_empty_both. apply AIs_ok_empty.
+	+ (* BR *) apply (AI_ok_instr _ _ (BR v_l') (mk_functype ts ts3_comp1)).
+		subst. apply (br v_C v_l' ts1' (lookup_total (C_LABELS v_C) v_l') ts3_comp1).
+
+	  	move: H3 => /leP Hbool. auto.
+		split => //.
+Qed.
+
+Lemma Step_pure__frame_vals_preserves : forall v_S v_C (v_n : n) (v_f : frame) (v_val : (list val)) v_func_type,
+	Admin_instrs_ok v_S v_C [(AI_FRAME_ v_n v_f (map fun_coec_val__admininstr v_val))] v_func_type ->
+	Step_pure [(AI_FRAME_ v_n v_f (map fun_coec_val__admininstr v_val))] (map fun_coec_val__admininstr v_val) ->
+	Admin_instrs_ok v_S v_C (map fun_coec_val__admininstr v_val) v_func_type.
+Proof.
+	move => v_S v_C v_n v_f v_val v_func_type HType HReduce.
+	destruct v_func_type as [ts1 ts2].
+	rewrite <- admin_instrs_ok_eq in HType.
+	apply Frame_typing in HType; destruct HType as [ts [? [? ?]]].
+	inversion H0. destruct H2.
+	apply Val_Const_list_typing in H3; simpl in *; subst.
+	apply admin_instrs_weakening_empty_1.
+	rewrite H3.
+	apply Const_list_typing_empty.
+Qed.
+
+Lemma Step_pure__return_frame_preserves : forall v_S v_C (v_n : n) (v_f : frame) (v_val' : (list val)) (v_val : (list val)) (v_instr : (list instr)) v_func_type,
+	Admin_instrs_ok v_S v_C [(AI_FRAME_ v_n v_f (@app _ (map fun_coec_val__admininstr v_val') (@app _ (map fun_coec_val__admininstr v_val) (@app _ [(AI_RETURN )] (map fun_coec_instr__admininstr v_instr)))))] v_func_type ->
+	Step_pure [(AI_FRAME_ v_n v_f (@app _ (map fun_coec_val__admininstr v_val') (@app _ (map fun_coec_val__admininstr v_val) (@app _ [(AI_RETURN )] (map fun_coec_instr__admininstr v_instr)))))] (map fun_coec_val__admininstr v_val) ->
+	((List.length v_val) = v_n) ->
+	Admin_instrs_ok v_S v_C (map fun_coec_val__admininstr v_val) v_func_type.
+Proof.
+	move => v_S v_C v_n v_f v_val' v_val v_instr v_func_type HType HReduce H.
+	destruct v_func_type as [ts1 ts2].
+	rewrite <- admin_instrs_ok_eq in HType.
+	apply Frame_typing in HType; destruct HType as [ts [? [? ?]]].
+	inversion H1; destruct H3.
+	apply_composition_typing H4.
+	apply_composition_typing H4_comp.
+	apply_composition_typing H4_comp0.
+	repeat rewrite <- app_right_nil in *.
+	rewrite <- admin_instrs_ok_eq in H3_comp1.
+	apply Val_Const_list_typing in H3_comp.
+	apply Val_Const_list_typing in H3_comp0.
+	apply empty_append in H1_comp; destruct H1_comp.
+	subst. simpl in *.
+	apply Return_typing in H3_comp1; destruct H3_comp1 as [ts0 [ts' [? ?]]].
+	subst.
+	inversion H3.
+Admitted. (*
+    destruct H0 as [? [? ?]].
+	subst.
+	inversion H7.
+	subst. simpl in *. rewrite _append_option_none_left in H2.
+	rewrite _append_option_none in H2.
+	injection H2 as ?; subst.
+	clear H4.
+	repeat rewrite -> app_assoc in H1_comp1.
+	eapply concat_cancel_last_n in H1_comp1; destruct H1_comp1.
+	rewrite <- H4.
+	apply admin_instrs_weakening_empty_1.
+	apply Const_list_typing_empty.
+	rewrite List.map_length.
+	rewrite H.
+	by destruct ts0.
+Qed. *)
+
+Lemma Step_pure__return_label_preserves : forall v_S v_C (v_n : n) (v_instr' : (list instr)) (v_val : (list val)) (v_instr : (list instr)) v_func_type,
+	Admin_instrs_ok v_S v_C [(AI_LABEL_ v_n v_instr' (@app _ (map fun_coec_val__admininstr v_val) (@app _ [(AI_RETURN )] (map fun_coec_instr__admininstr v_instr))))] v_func_type ->
+	Step_pure [(AI_LABEL_ v_n v_instr' (@app _ (map fun_coec_val__admininstr v_val) (@app _ [(AI_RETURN )] (map fun_coec_instr__admininstr v_instr))))] (@app _ (map fun_coec_val__admininstr v_val) [(AI_RETURN )]) ->
+	Admin_instrs_ok v_S v_C (@app _ (map fun_coec_val__admininstr v_val) [(AI_RETURN )]) v_func_type.
+Proof.
+	move => v_S v_C v_n v_instr' v_val v_instr v_func_type HType HReduce.
+	destruct v_func_type as [ts1 ts2].
+	rewrite <- admin_instrs_ok_eq in HType.
+	apply Label_typing in HType; destruct HType as [ts [ts2' [? [? [? ?]]]]].
+	apply_composition_typing H2.
+	apply_composition_typing H4_comp.
+	repeat rewrite <- app_right_nil in *.
+	rewrite <- admin_instrs_ok_eq in H3_comp0.
+	apply Return_typing in H3_comp0; destruct H3_comp0 as [ts0 [ts' [? ?]]].
+	unfold upd_label, set in H1. simpl in H1.
+	apply Val_Const_list_typing in H3_comp.
+	apply empty_append in H1_comp; destruct H1_comp.
+	subst. simpl in *.
+	apply admin_instrs_weakening_empty_1.
+	eapply admin_composition'.
+	apply Const_list_typing_empty.
+	rewrite H1_comp0.
+	rewrite H2_comp.
+	apply AIs_ok_frame.
+	rewrite <- admin_instrs_ok_eq.
+	apply AI_ok_instr with (v_instr := RETURN).
+	by apply res_return.
+Qed.
+
+Lemma Step_pure__trap_vals_preserves : forall v_S v_C (v_val : (list val)) (v_admininstr : (list admininstr)) v_func_type,
+	Admin_instrs_ok v_S v_C (@app _ (map fun_coec_val__admininstr v_val) (@app _ [(AI_TRAP )] v_admininstr)) v_func_type ->
+	((v_val <> []) \/ (v_admininstr <> [])) ->
+	Admin_instrs_ok v_S v_C [(AI_TRAP )] v_func_type.
+Proof.
+	move => v_S v_C v_val v_instr v_func_type HType H.
+	destruct v_func_type as [ts1 ts2].
+	rewrite <- admin_instrs_ok_eq.
+	apply AI_ok_trap.
+Qed.
+
+Lemma Step_pure__trap_label_preserves : forall v_S v_C (v_n : n) (v_instr' : (list instr)) v_func_type,
+	Admin_instrs_ok v_S v_C [(AI_LABEL_ v_n v_instr' [(AI_TRAP )])] v_func_type ->
+	Admin_instrs_ok v_S v_C [(AI_TRAP )] v_func_type.
+Proof.
+	move => v_S v_C n v_instr' v_func_type HType.
+	destruct v_func_type as [ts1 ts2].
+	rewrite <- admin_instrs_ok_eq.
+	apply AI_ok_trap.
+Qed.
+
+Lemma Step_pure__trap_frame_preserves : forall v_S v_C (v_n : n) (v_f : frame) v_func_type,
+	Admin_instrs_ok v_S v_C [(AI_FRAME_ v_n v_f [(AI_TRAP )])] v_func_type ->
+	Admin_instrs_ok v_S v_C [(AI_TRAP )] v_func_type.
+Proof.
+	intros.
+	destruct v_func_type as [ts1 ts2].
+	rewrite <- admin_instrs_ok_eq.
+	apply AI_ok_trap.
+Qed.
+
+Lemma Step_pure__unop_val_preserves : forall v_S v_C (v_t : valtype) (v_c_1 : val_ v_t) (v_unop : unop_ v_t) v_c v_func_type,
+	Admin_instrs_ok v_S v_C [(AI_CONST v_t v_c_1);(AI_UNOP v_t v_unop)] v_func_type ->
+	Step_pure [(AI_CONST v_t v_c_1);(AI_UNOP v_t v_unop)] [(AI_CONST v_t v_c)] ->
+	Admin_instrs_ok v_S v_C [(AI_CONST v_t v_c)] v_func_type.
+Proof.
+	move => v_S v_C t v unop_op v_c tf HType HReduce.
+	destruct tf as [tf1 tf2].
+	rewrite -cat1s in HType; subst.
+	apply admin_composition_typing_single in HType; destruct HType as [ts1 [ts2 [ts3 [ts4 [H1 [H3 [H4 H5]]]]]]].
+	rewrite -> app_left_single_nil in H4; subst.
+	apply admin_composition_typing_single in H4; destruct H4 as [ts5 [ts6 [ts7 [ts8 [H6 [H7 [H8 H9]]]]]]].
+	apply AI_const_typing in H9.
+	apply Unop_typing in H5; destruct H5 as [H10 [ts H11]]. 
+	apply admin_empty_same_type in H8; subst.
+	repeat rewrite app_assoc.
+	apply admin_instrs_weakening_empty_1.
+	apply (AIs_ok_seq v_S v_C [] (AI_CONST t v_c) [] [t] []).
+	apply AIs_ok_empty.
+	apply (AI_ok_instr v_S v_C (CONST t v_c) (mk_functype [] [t])).
+	by apply const.
+Qed.
+
+Lemma Step_pure__unop_trap_preserves : forall v_S v_C (v_t : valtype) (v_c_1 : val_ v_t) (v_unop : unop_ v_t) v_func_type,
+	Admin_instrs_ok v_S v_C [(AI_CONST v_t v_c_1);(AI_UNOP v_t v_unop)] v_func_type ->
+	Step_pure [(AI_CONST v_t v_c_1);(AI_UNOP v_t v_unop)] [(AI_TRAP )] ->
+	Admin_instrs_ok v_S v_C [(AI_TRAP )] v_func_type.
+Proof.
+	move => v_S v_C v_t v_c_1 v_unop v_func_type HType HReduce.
+	destruct v_func_type as [tf1 tf2].
+	apply (AIs_ok_seq v_S v_C [] (AI_TRAP) tf1 tf2 tf1).
+	- (* Empty *) apply admin_weakening_empty_both. apply AIs_ok_empty.
+	- (* TRAP *) apply AI_ok_trap.
+Qed.
+
+
+Lemma Step_pure__binop_val_preserves : forall v_S v_C (v_t : valtype) (v_c_1 : val_ v_t) (v_c_2 : val_ v_t) (v_binop : binop_ v_t) v_c v_func_type,
+	Admin_instrs_ok v_S v_C [(AI_CONST v_t v_c_1);(AI_CONST v_t v_c_2);(AI_BINOP v_t v_binop)] v_func_type ->
+	Step_pure [(AI_CONST v_t v_c_1);(AI_CONST v_t v_c_2);(AI_BINOP v_t v_binop)] [(AI_CONST v_t v_c)] ->
+	Admin_instrs_ok v_S v_C [(AI_CONST v_t v_c)] v_func_type.
+Proof.
+	move => v_S v_C v_t v_c_1 v_c_2 v_binop v_c v_func_type HType HReduce.
+	destruct v_func_type as [tf1 tf2].
+	apply_composition_typing_and_single HType.
+	apply_composition_typing_and_single H4_comp.
+	apply_composition_typing_single H4_comp1.
+	apply AI_const_typing in H4_comp0.
+	apply AI_const_typing in H4_comp.
+	apply Binop_typing in H4_comp2; destruct H4_comp2 as [H [ts H0]].
+	subst.
+	repeat rewrite -> app_assoc in H1_comp0.
+	apply split_append_last in H1_comp0; destruct H1_comp0.
+	rewrite H in H1_comp1.
+	repeat rewrite -> app_assoc in H1_comp1.
+	apply split_append_last in H1_comp1; destruct H1_comp1.
+	rewrite H1.
+	repeat rewrite -> app_assoc.
+	apply admin_instrs_weakening_empty_1.
+	apply (AIs_ok_seq v_S v_C [] (AI_CONST v_t v_c) [] [v_t] []).
+	apply AIs_ok_empty.
+	apply (AI_ok_instr v_S v_C (CONST v_t v_c) (mk_functype [] [v_t])).
+	by apply const.
+Qed.
+
+Lemma Step_pure__binop_trap_preserves : forall v_S v_C (v_t : valtype) v_c_1 v_c_2 v_binop v_func_type,
+	Admin_instrs_ok v_S v_C [(AI_CONST v_t v_c_1);(AI_CONST v_t v_c_2);(AI_BINOP v_t v_binop)] v_func_type ->
+	Step_pure [(AI_CONST v_t v_c_1);(AI_CONST v_t v_c_2);(AI_BINOP v_t v_binop)] [(AI_TRAP )] ->
+	Admin_instrs_ok v_S v_C [(AI_TRAP )] v_func_type.
+Proof.
+	move => v_S v_C v_t v_c_1 v_c_2 v_binop v_func_type HType HReduce.
+	destruct v_func_type as [tf1 tf2].
+	apply (AIs_ok_seq v_S v_C [] (AI_TRAP) tf1 tf2 tf1).
+	- (* Empty *) apply admin_weakening_empty_both. apply AIs_ok_empty.
+	- (* TRAP *) apply AI_ok_trap.
+Qed.
+
+
+
+Lemma Step_pure__testop_preserves : forall v_S v_C (v_t : valtype) v_c_1 (v_testop : testop_ v_t) (v_c : iN 32) v_func_type,
+	Admin_instrs_ok v_S v_C [(AI_CONST v_t v_c_1);(AI_TESTOP v_t v_testop)] v_func_type ->
+	Step_pure [(AI_CONST v_t v_c_1);(AI_TESTOP v_t v_testop)] [(AI_CONST I32 v_c)] ->
+	Admin_instrs_ok v_S v_C [(AI_CONST I32 v_c)] v_func_type.
+Proof.
+	move => v_S v_C v_t v_c_1 v_testop v_c v_func_type HType HReduce.
+	destruct v_func_type as [tf1 tf2].
+	apply_composition_typing_and_single HType.
+	apply_composition_typing_single H4_comp.
+	apply AI_const_typing in H4_comp0.
+	apply Testop_typing in H4_comp1; destruct H4_comp1 as [ts [H1 H2]]; subst.
+	repeat rewrite -> app_assoc in H1_comp1. apply split_append_last in H1_comp1; destruct H1_comp1; subst.
+	rewrite H.
+	repeat rewrite -> app_assoc.
+	apply admin_instrs_weakening_empty_1.
+	apply (AIs_ok_seq v_S v_C [] (AI_CONST (I32) v_c) [] [I32] []). 
+	- (* Empty *) apply AIs_ok_empty.
+	- (* Const *) apply (AI_ok_instr v_S v_C (CONST (I32) v_c) (mk_functype [] [I32])).
+		by apply const.
+Qed.
+
+Lemma Step_pure__relop_preserves : forall v_S v_C (v_t : valtype) v_c_1 v_c_2 (v_relop : relop_ v_t) (v_c : iN 32) v_func_type,
+	Admin_instrs_ok v_S v_C [(AI_CONST v_t v_c_1);(AI_CONST v_t v_c_2);(AI_RELOP v_t v_relop)] v_func_type ->
+	Step_pure [(AI_CONST v_t v_c_1);(AI_CONST v_t v_c_2);(AI_RELOP v_t v_relop)] [(AI_CONST I32 v_c)] ->
+	Admin_instrs_ok v_S v_C [(AI_CONST I32 v_c)] v_func_type.
+Proof.
+	move => v_S v_C v_t v_c_1 v_c_2 v_relop v_c v_func_type HType HReduce.
+	destruct v_func_type as [tf1 tf2].
+	apply_composition_typing_and_single HType.
+	apply_composition_typing_and_single H4_comp.
+	apply_composition_typing_single H4_comp1.
+	apply AI_const_typing in H4_comp0.
+	apply AI_const_typing in H4_comp.
+	apply Relop_typing in H4_comp2; destruct H4_comp2 as [ts [H1 H2]].
+	subst.
+	rewrite split_cons in H1_comp0.
+	repeat rewrite -> app_assoc in H1_comp0; apply split_append_last in H1_comp0; destruct H1_comp0.
+	rewrite H in H1_comp1.
+	repeat rewrite -> app_assoc in H1_comp1; apply split_append_last in H1_comp1; destruct H1_comp1.
+	rewrite H1.
+	repeat rewrite -> app_assoc.
+	apply admin_instrs_weakening_empty_1.
+	apply (AIs_ok_seq v_S v_C [] (AI_CONST (I32) v_c) [] [I32] []).
+	- (* Empty *) apply AIs_ok_empty.
+	- (* Const *) apply (AI_ok_instr v_S v_C (CONST (I32) v_c) (mk_functype [] [I32])).
+	by apply const.
+Qed.
+
+Lemma Step_pure__cvtop_val_preserves : forall v_S v_C (v_t_1 : valtype) v_c_1 (v_t_2 : valtype) (v_cvtop : cvtop) (v_sx : (option sx)) v_c v_func_type,
+	Admin_instrs_ok v_S v_C [(AI_CONST v_t_1 v_c_1);(AI_CVTOP v_t_2 v_t_1 v_cvtop)] v_func_type ->
+	Step_pure [(AI_CONST v_t_1 v_c_1);(AI_CVTOP v_t_2 v_t_1 v_cvtop)] [(AI_CONST v_t_2 v_c)] ->
+	Admin_instrs_ok v_S v_C [(AI_CONST v_t_2 v_c)] v_func_type.
+Proof.
+	move => v_S v_C v_t_1 v_c_1 v_t_2 v_cvtop v_sx v_c v_func_type HType HReduce.
+	destruct v_func_type as [tf1 tf2].
+	apply_composition_typing_and_single HType.
+	apply_composition_typing_single H4_comp.
+	apply AI_const_typing in H4_comp0.
+	apply Cvtop_typing in H4_comp1; destruct H4_comp1 as [ts [H1 H2]].
+	subst.
+	repeat rewrite -> app_assoc in H1_comp1; apply split_append_last in H1_comp1; destruct H1_comp1.
+	rewrite H.
+	repeat rewrite -> app_assoc.
+	apply admin_instrs_weakening_empty_1.
+	apply (AIs_ok_seq v_S v_C [] (AI_CONST v_t_2 v_c) [] [v_t_2] []).
+	- (* Empty *) apply AIs_ok_empty.
+	- (* Const *) apply (AI_ok_instr v_S v_C (CONST v_t_2 v_c) (mk_functype [] [v_t_2])).
+	by apply const.
+Qed.
+
+Lemma Step_pure__cvtop_trap_preserves : forall v_S v_C (v_t_1 : valtype) v_c_1 (v_t_2 : valtype) (v_cvtop : cvtop) (v_sx : (option sx)) v_func_type,
+	Admin_instrs_ok v_S v_C [(AI_CONST v_t_1 v_c_1);(AI_CVTOP v_t_2 v_t_1 v_cvtop)] v_func_type ->
+	Step_pure [(AI_CONST v_t_1 v_c_1);(AI_CVTOP v_t_2 v_t_1 v_cvtop)] [(AI_TRAP )] ->
+	Admin_instrs_ok v_S v_C [(AI_TRAP )] v_func_type.
+Proof.
+	move => v_S v_C v_t_1 v_c_1 v_t_2 v_cvtop v_sx v_func_type HType HReduce.
+	destruct v_func_type as [tf1 tf2].
+	apply (AIs_ok_seq v_S v_C [] (AI_TRAP) tf1 tf2 tf1).
+	- (* Empty *) apply admin_weakening_empty_both. apply AIs_ok_empty.
+	- (* TRAP *) apply AI_ok_trap.
+Qed.
+
+Lemma Step_pure__local_tee_preserves : forall v_S v_C (v_val : val) (v_x : idx) v_func_type,
+	Admin_instrs_ok v_S v_C [(v_val : admininstr);(AI_LOCAL_TEE v_x)] v_func_type ->
+	Step_pure [(v_val : admininstr);(AI_LOCAL_TEE v_x)] [(v_val : admininstr);(v_val : admininstr);(AI_LOCAL_SET v_x)] ->
+	Admin_instrs_ok v_S v_C [(v_val : admininstr);(v_val : admininstr);(AI_LOCAL_SET v_x)] v_func_type.
+Proof.
+	move => v_S v_C v_val v_x v_func_type HType HReduce.
+	destruct v_func_type as [tf1 tf2].
+	apply_composition_typing_and_single HType.
+	apply_composition_typing_single H4_comp.
+	induction v_val.
+	apply AI_const_typing in H4_comp0.
+	apply Local_tee_typing in H4_comp1; destruct H4_comp1 as [ts [t [H1 [H2 [H3 H4]]]]].
+	subst.
+	repeat rewrite -> app_assoc in H1_comp1; apply split_append_last in H1_comp1; destruct H1_comp1.
+	rewrite H.
+	repeat rewrite -> app_assoc.
+	apply admin_instrs_weakening_empty_1.
+	unfold fun_coec_val__admininstr.
+	rewrite <- H0.
+	apply (AIs_ok_seq v_S v_C [AI_CONST v_valtype v_val_; AI_CONST v_valtype v_val_] 
+		(AI_LOCAL_SET v_x) [] [v_valtype] ([v_valtype] ++ [v_valtype])).
+	apply (AIs_ok_seq v_S v_C [AI_CONST v_valtype v_val_] 
+		(AI_CONST v_valtype v_val_) [] ([v_valtype] ++ [v_valtype]) [v_valtype]).
+	apply (AIs_ok_seq v_S v_C [] 
+	(AI_CONST v_valtype v_val_) [] [v_valtype] []).
+	- (* Empty *) apply AIs_ok_empty.
+	- (* Const 1 *) apply (AI_ok_instr v_S v_C (CONST v_valtype v_val_) (mk_functype [] [v_valtype])).
+		apply const.
+	- (* Const 2 *) apply admin_instr_weakening_empty_1. 
+		apply (AI_ok_instr v_S v_C (CONST v_valtype v_val_) (mk_functype [] [v_valtype])).
+		apply const.
+	- (* Set *) apply admin_instr_weakening_empty_2. 
+		apply (AI_ok_instr v_S v_C (LOCAL_SET v_x) (mk_functype [v_valtype] [])).
+		apply local_set.
+		move : H3 => /leP Hbool. auto. auto.
+Qed.
+
+Lemma Step_read__block_preserves : forall v_S (r_v_f : frame) v_C (v_z : state) (v_t : (option valtype)) (v_instr : (list instr)) (v_n : n) v_func_type v_t1 lab ret ,
+	Admin_instrs_ok v_S (upd_label (upd_local_return v_C (v_t1 ++ C_LOCALS v_C) ret) lab)[(AI_BLOCK v_t v_instr)] v_func_type ->
+	Module_instance_ok v_S (F_MODULE r_v_f) v_C  ->
+	v_z = mk_state v_S r_v_f ->
+	(((v_t = None) /\ (v_n = 0)) \/ ((v_t <> None) /\ (v_n = 1))) ->
+	Forall2 (fun v_t v_val => Val_ok v_val v_t) v_t1 (LOCALS r_v_f) ->
+	Admin_instrs_ok v_S (upd_label (upd_local_return v_C (v_t1 ++ C_LOCALS v_C) ret) lab) [(AI_LABEL_ v_n [] (map fun_coec_instr__admininstr v_instr))] v_func_type.
+Proof.
+	move => v_S r_v_f v_C v_z v_t v_instr v_n v_func_type v_t1 lab ret HType HMinst HState H1 HValOK.
+	destruct v_func_type as [ts1 ts2].
+	rewrite <- admin_instrs_ok_eq in HType.
+	apply Block_typing in HType; destruct HType as [ts [? [? ?]]]; subst. simpl in H2.
+	rewrite <- admin_instrs_ok_eq.
+	apply admin_instr_weakening_empty_1.
+	apply AI_ok_label with (v_t_1 := v_t).
+	repeat split => //=.
+	apply instrs_weakening_empty_both.
+	Check instrs_empty.
+	apply instrs_empty.
+	apply AIs_ok_instrs with (v_S := v_S) in H2.
+	apply H2.
+	destruct H1; destruct H => //=; subst => //=.
+	destruct v_t => //=.
+Qed.
+
+Lemma Step_read__loop_preserves : forall v_S (r_v_f : frame) v_C (v_z : state) (v_t : (option valtype)) (v_instr : (list instr)) v_func_type v_t1 lab ret ,
+	Admin_instrs_ok v_S (upd_label (upd_local_return v_C (v_t1 ++ C_LOCALS v_C) ret) lab)[(AI_LOOP v_t v_instr)] v_func_type ->
+	Module_instance_ok v_S (F_MODULE r_v_f) v_C  ->
+	v_z = mk_state v_S r_v_f ->
+	Forall2 (fun v_t v_val => Val_ok v_val v_t) v_t1 (LOCALS r_v_f) ->
+	Admin_instrs_ok v_S (upd_label (upd_local_return v_C (v_t1 ++ C_LOCALS v_C) ret) lab) [(AI_LABEL_ 0 [(LOOP v_t v_instr)] (map fun_coec_instr__admininstr v_instr))] v_func_type.
+Proof.
+	move => v_S r_v_f v_C v_z v_t v_instr v_func_type v_t1 lab ret HType HMinst H HValOK.
+	destruct v_func_type as [ts1 ts2].
+	rewrite <- admin_instrs_ok_eq in HType.
+	apply Loop_typing in HType; destruct HType as [ts [? [? ?]]]; subst.
+	simpl in H2.
+	rewrite <- admin_instrs_ok_eq.
+	apply admin_instr_weakening_empty_1.
+	apply AI_ok_label with (v_t_1 := None).
+	repeat split => //=.
+	- simpl.
+		rewrite app_left_single_nil.
+		apply (instrs_seq _ [] (LOOP v_t v_instr) [] v_t []).
+		- apply instrs_empty.
+		- apply loop.
+(* TODO *)
+Admitted.
+(*
+		apply H2. 
+	- apply AIs_ok_instrs with (v_S := v_S) in H2.
+		apply H2. auto.
+Qed. *)
+
+Lemma Step_read__call_preserves : forall v_S (r_v_f : frame) v_C (v_z : state) (v_x : idx) v_func_type v_t1 lab ret ,
+	Admin_instrs_ok v_S (upd_label (upd_local_return v_C (v_t1 ++ C_LOCALS v_C) ret) lab)[(AI_CALL v_x)] v_func_type ->
+	Module_instance_ok v_S (F_MODULE r_v_f) v_C  ->
+	v_z = mk_state v_S r_v_f ->
+	(v_x < (List.length (fun_funcaddr v_z)))%coq_nat ->
+	Forall2 (fun v_t v_val => Val_ok v_val v_t) v_t1 (LOCALS r_v_f) ->
+	Admin_instrs_ok v_S (upd_label (upd_local_return v_C (v_t1 ++ C_LOCALS v_C) ret) lab) [(AI_CALL_ADDR (lookup_total (fun_funcaddr v_z) v_x))] v_func_type.
+Proof.
+	move => v_S r_v_f v_C v_z v_x v_func_type v_t1 lab ret HType HMinst H H1 HValOK.
+	destruct v_func_type as [ts1 ts2].
+	rewrite <- admin_instrs_ok_eq in HType.
+	apply Call_typing in HType; destruct HType as [ts [t1s' [t2s' [? [? [? ?]]]]]]; subst.
+	simpl in *.
+	apply AIs_ok_frame.
+	rewrite <- admin_instrs_ok_eq.
+	eapply AI_ok_call_addr.
+	inversion HMinst.
+	simpl in *.
+	rewrite <- H in H1. simpl in H1.
+	apply Forall2_lookup in H5. destruct H5.
+	apply H15 in H1. rewrite <- H2. rewrite <- H14.
+	apply H1.
+Qed.
+
+Lemma tc_func_reference2: forall v_S v_C v_minst idx tf v_type,
+  lookup_total (MODULE_TYPES v_minst) idx = FUNC_TYPE v_type ->
+  Module_instance_ok v_S v_minst v_C ->
+  lookup_total (C_TYPES v_C) idx = tf ->
+  tf = FUNC_TYPE v_type.
+Proof.
+	move => v_S v_C v_minst idx tf v_type H HMinst H1.
+	inversion HMinst. subst. simpl in *. auto.
+Qed.
+
+
+Lemma store_typed_exterval_types: forall v_S v_f v_a,
+	(v_a < List.length (FUNCS v_S))%coq_nat ->
+	lookup_total (FUNCS v_S) v_a = v_f ->
+    Store_ok v_S ->
+    Externaddrs_ok v_S (EXTVAL_FUNC v_a) (EXT_FUNC (FUNC_TYPE v_f)).
+Proof.
+	move => v_S v_f v_a HLength H HST.
+	inversion HST; subst; simpl in *.
+	
+	apply Forall2_lookup in H2; destruct H2.
+	apply H0 in HLength as HFunc.
+	simpl in *.
+	inversion HFunc; subst; simpl in *.
+	apply extaddr_ok_func with (v_minst := v_moduleinst) (v_func := v_func).
+	- move/ltP: HLength => Hprop. auto.
+	- simpl in *. auto.
+Qed.
+
+Lemma Step_read__call_indirect_call_preserves : forall v_S (r_v_f : frame) v_C (v_z : state) (v_i : nat) (v_x : idx) (v_a : addr) v_func_type v_t1 lab ret ,
+	Admin_instrs_ok v_S (upd_label (upd_local_return v_C (v_t1 ++ C_LOCALS v_C) ret) lab)[(AI_CONST I32 (fun_nat__u32 v_i));(AI_CALL_INDIRECT v_x)] v_func_type ->
+	Module_instance_ok v_S (F_MODULE r_v_f) v_C  ->
+	Store_ok v_S ->
+	v_z = mk_state v_S r_v_f ->
+	(v_i < (List.length (REFS (fun_table v_z 0))))%coq_nat ->
+	(v_a < (List.length (fun_funcinst v_z)))%coq_nat ->
+	((lookup_total (REFS (fun_table v_z 0)) v_i) = (Some v_a)) ->
+	((fun_type v_z v_x) = (FUNC_TYPE (lookup_total (fun_funcinst v_z) v_a))) ->
+	Forall2 (fun v_t v_val => Val_ok v_val v_t) v_t1 (LOCALS r_v_f) ->
+	Admin_instrs_ok v_S (upd_label (upd_local_return v_C (v_t1 ++ C_LOCALS v_C) ret) lab) [(AI_CALL_ADDR v_a)] v_func_type.
+Proof.
+	move => v_S r_v_f v_C v_z v_i v_x v_a v_func_type v_t1 lab ret HType HMinst HST H1 H2 H3 H4 H5 HValOK.
+	destruct v_func_type as [ts1 ts2].
+	apply_composition_typing_and_single HType.
+	apply AI_const_typing in H4_comp0.
+	rewrite <- admin_instrs_ok_eq in H4_comp.
+	apply Call_indirect_typing in H4_comp; destruct H4_comp as [tn [tm [ts [? [? [? ?]]]]]]; subst.
+	repeat rewrite -> app_assoc in H1. apply split_append_last in H1; destruct H1.
+	rewrite H1.
+	repeat rewrite -> app_assoc.
+	apply AIs_ok_frame.
+	rewrite <- admin_instrs_ok_eq.
+	apply AI_ok_call_addr.
+	unfold fun_table in H4.
+	unfold fun_type in H5.
+	unfold fun_table in H2.
+	simpl in *.
+	assert ((mk_functype tn tm) = FUNC_TYPE (lookup_total (FUNCS v_S) v_a)) as HFType; first by eapply tc_func_reference2; eauto.
+	rewrite -> HFType.
+	eapply store_typed_exterval_types; eauto.
+Qed.
+
+Lemma Step_read__call_indirect_trap_preserves : forall v_S (r_v_f : frame) v_C (v_z : state) (v_i : val_ I32) (v_x : idx) v_func_type v_t1 lab ret ,
+	Admin_instrs_ok v_S (upd_label (upd_local_return v_C (v_t1 ++ C_LOCALS v_C) ret) lab)[(AI_CONST I32 v_i);(AI_CALL_INDIRECT v_x)] v_func_type ->
+	Module_instance_ok v_S (F_MODULE r_v_f) v_C  ->
+	v_z = mk_state v_S r_v_f ->
+	(~(Step_read_before_call_indirect_trap (mk_config v_z [(AI_CONST I32 v_i);(AI_CALL_INDIRECT v_x)]))) ->
+	Forall2 (fun v_t v_val => Val_ok v_val v_t) v_t1 (LOCALS r_v_f) ->
+	Admin_instrs_ok v_S (upd_label (upd_local_return v_C (v_t1 ++ C_LOCALS v_C) ret) lab) [(AI_TRAP )] v_func_type.
+Proof.
+	intros.
+	destruct v_func_type.
+	rewrite <- admin_instrs_ok_eq.
+	apply AI_ok_trap.
+Qed.
+
+Lemma Step_read__call_addr_preserves : forall v_S (r_v_f : frame) v_C (v_z : state) (v_val : (list val)) (v_k : nat) (v_a : addr) (v_n : n) (v_f : frame) (v_instr : (list instr)) (v_t_1 : (list valtype)) (v_t_2 : resulttype) (v_mm : moduleinst) (v_func : func) (v_x : idx) (v_t : (list valtype)) v_func_type v_t1 lab ret ,
+	Admin_instrs_ok v_S (upd_label (upd_local_return v_C (v_t1 ++ C_LOCALS v_C) ret) lab)(@app _ (map fun_coec_val__admininstr v_val) [(AI_CALL_ADDR v_a)]) v_func_type ->
+	Module_instance_ok v_S (F_MODULE r_v_f) v_C  ->
+	Store_ok v_S -> 
+	Datatypes.length v_val = Datatypes.length v_t_1 -> 
+	v_z = mk_state v_S r_v_f ->
+	(v_a < (List.length (fun_funcinst v_z)))%coq_nat ->
+	((lookup_total (fun_funcinst v_z) v_a) = {| FUNC_TYPE := (mk_functype v_t_1 v_t_2); FUNC_MODULE := v_mm; CODE := v_func |}) ->
+	(v_n = fun_optionSize v_t_2) ->
+	(v_func = (FUNC v_x (List.map (fun v_t => (LOCAL v_t)) (v_t)) v_instr)) ->
+	(v_f = {| LOCALS := (@app _ v_val (List.map (fun v_t => (fun_default_ v_t)) (v_t))); F_MODULE := v_mm |}) ->
+	Forall2 (fun v_t v_val => Val_ok v_val v_t) v_t1 (LOCALS r_v_f) ->
+	Admin_instrs_ok v_S (upd_label (upd_local_return v_C (v_t1 ++ C_LOCALS v_C) ret) lab) [(AI_FRAME_ v_n v_f [(AI_LABEL_ v_n [] (map fun_coec_instr__admininstr v_instr))])] v_func_type.
+Admitted.
+(* Proof.
+	move => v_S r_v_f v_C v_z v_val v_k v_a v_n v_f v_instr v_t_1 v_t_2 v_mm v_func v_x v_t v_func_type v_t1 lab ret HType HMinst H1 H2 H3 H4 H5 H6 H7 H8 H9.
+	destruct v_func_type as [ts1 ts2].
+	apply_composition_typing_single HType.
+	apply Val_Const_list_typing in H3_comp.
+	rewrite -> H3 in H4. simpl in H4.
+	rewrite -> H3 in H5. simpl in H5.
+	eapply CALL_ADDR_invoke_typing with (v_t_1 := v_t_1) (v_t_2 := v_t_2) (v_mm := v_mm) in H4_comp; eauto;
+	try apply H5. 
+	destruct H4_comp as [ts' [C' [? [? [??]]]]].
+	subst.
+	apply concat_cancel_last_n in H; last by (repeat rewrite length_is_size in H2; rewrite List.map_length).
+	destruct H; subst.
+	repeat rewrite -> app_assoc.
+	apply admin_instrs_weakening_empty_1.
+	rewrite <- admin_instrs_ok_eq.
+	apply AI_ok_frame. auto. split => //=.
+	eapply Thread_ok__. split. 
+	apply Frame_ok__ with (v_t := ((List.map typeof v_val) ++ v_t)). repeat split => //=.
+	repeat rewrite -> List.app_length.
+	repeat rewrite -> List.map_length => //=.
+	apply H10.
+	apply Forall2_Val_ok_is_same_as_map.
+	rewrite List.map_app.
+	rewrite List.app_inv_head_iff.
+	apply typeof_default_inverse.
+	rewrite <- admin_instrs_ok_eq.
+	apply AI_ok_label with (v_t_1 := v_t_2); repeat split => //=.
+	- apply instrs_weakening_empty_both. apply instrs_empty.
+	- rewrite fold_append. simpl.
+		repeat rewrite _append_option_none_left.
+		apply AIs_ok_instrs.
+		apply H11. 
+Qed. *)
+
+Lemma Step_read__local_get_preserves : forall v_S (r_v_f : frame) v_C (v_z : state) (v_x : idx) v_func_type v_t1 lab ret ,
+	Admin_instrs_ok v_S (upd_label (upd_local_return v_C (v_t1 ++ C_LOCALS v_C) ret) lab)[(AI_LOCAL_GET v_x)] v_func_type ->
+	Module_instance_ok v_S (F_MODULE r_v_f) v_C  ->
+	v_z = mk_state v_S r_v_f ->
+	Forall2 (fun v_t v_val => Val_ok v_val v_t) v_t1 (LOCALS r_v_f) ->
+	Admin_instrs_ok v_S (upd_label (upd_local_return v_C (v_t1 ++ C_LOCALS v_C) ret) lab) [((fun_local v_z v_x) : admininstr)] v_func_type.
+Proof.
+	move => v_S r_v_f v_C v_z v_x v_func_type v_t1 lab ret HType HMinst H1 HValOK.
+	destruct v_func_type as [ts1 ts2].
+	rewrite <- admin_instrs_ok_eq.
+	rewrite <- admin_instrs_ok_eq in HType.
+	apply Get_local_typing in HType; destruct HType as [t [? [? ?]]]. 
+	simpl in *.
+	subst.
+	apply admin_instr_weakening_empty_1.
+	unfold fun_local.
+	apply inst_t_context_local_empty in HMinst.
+	rewrite HMinst in H2.
+	rewrite HMinst.
+	apply Forall2_lookup in HValOK; destruct HValOK.
+	rewrite <- app_right_nil in H2.
+	rewrite <- app_right_nil.
+	apply H0 in H2. 
+	inversion H2.
+	subst.
+	unfold fun_localidx__nat in H3 at 2.
+	unfold fun_proj_uN_0.
+	rewrite <- H3.
+	apply (AI_ok_instr v_S (upd_label (upd_local_return v_C v_t1 ret) lab)
+	(CONST (@lookup_total valtype Inhabited__valtype v_t1 (fun_localidx__nat v_x)) v_c_t)
+	(mk_functype [] [(lookup_total v_t1 v_x)])).
+	apply const.
+Qed.
+
+Lemma global_type_reference: forall v_S v_i v_x v_C mut v t,
+    Module_instance_ok v_S v_i v_C ->
+	(v_x < Datatypes.length (C_GLOBALS v_C))%coq_nat -> 
+    (VALUE (lookup_total (GLOBALS v_S) (lookup_total (MODULE_GLOBALS v_i) v_x))) = v ->
+    lookup_total (C_GLOBALS v_C) v_x = mk_globaltype mut t ->
+    exists v_val_, typeof v = t /\ v = VAL_CONST t v_val_.
+Admitted.
+(* Proof.
+	move => v_S i v_x v_C mut v t HMinst HLength HVal HTypeLookup.
+	inversion HMinst; decomp; subst.
+	simpl in *.
+	apply Forall2_lookup2 in H9; destruct H9.
+	apply H1 in HLength.
+	inversion HLength; destruct H13.
+	rewrite H14.
+	simpl.
+	rewrite HTypeLookup in H12. injection H12 as ?; eauto.
+	exists v_val_.
+	split => //=.
+	f_equal => //=.
+Qed. *)
+
+Lemma Step_read__global_get_preserves : forall v_S (r_v_f : frame) v_C (v_z : state) (v_x : idx) v_func_type v_t1 lab ret ,
+	Admin_instrs_ok v_S (upd_label (upd_local_return v_C (v_t1 ++ C_LOCALS v_C) ret) lab)[(AI_GLOBAL_GET v_x)] v_func_type ->
+	Module_instance_ok v_S (F_MODULE r_v_f) v_C  ->
+	v_z = mk_state v_S r_v_f ->
+	Forall2 (fun v_t v_val => Val_ok v_val v_t) v_t1 (LOCALS r_v_f) ->
+	Admin_instrs_ok v_S (upd_label (upd_local_return v_C (v_t1 ++ C_LOCALS v_C) ret) lab) [((VALUE (fun_global v_z v_x)) : admininstr)] v_func_type.
+Proof.
+	move => v_S r_v_f v_C v_z v_x v_func_type v_t1 lab ret HType HMinst H HValOK.
+	destruct v_func_type as [ts1 ts2].
+	rewrite <- admin_instrs_ok_eq in HType.
+	rewrite <- admin_instrs_ok_eq.
+	apply Get_global_typing in HType.
+	destruct HType as [mut [t [? [? ?]]]].
+	simpl in *.
+	subst.
+	unfold fun_global.
+
+	remember ((VALUE
+	(lookup_total (GLOBALS v_S)
+	   (lookup_total (MODULE_GLOBALS (F_MODULE r_v_f)) (fun_proj_uN_0 32 v_x))))) as v.
+	eapply global_type_reference in HMinst; eauto; destruct HMinst as [v_val_ [? ?]].
+	rewrite H1 in Heqv.
+	apply admin_instr_weakening_empty_1.
+	rewrite Heqv.
+	eapply (AI_ok_instr v_S _ (CONST t v_val_) (mk_functype [] [t])).
+	apply const.
+Qed.
+
+Lemma Step_read__load_num_trap_preserves : forall v_S (r_v_f : frame) v_C (v_z : state) (v_i : nat) (v_t : valtype) (v_mo : memarg) v_func_type v_t1 lab ret ,
+	Admin_instrs_ok v_S (upd_label (upd_local_return v_C (v_t1 ++ C_LOCALS v_C) ret) lab)[(AI_CONST I32 (fun_nat__u32 v_i : val_ I32));(AI_LOAD v_t None v_mo)] v_func_type ->
+	Module_instance_ok v_S (F_MODULE r_v_f) v_C  ->
+	v_z = mk_state v_S r_v_f ->
+	(((v_i + (OFFSET v_mo)) + ((fun_size v_t) / 8)) > (List.length (BYTES (fun_mem v_z 0))))%coq_nat ->
+	Forall2 (fun v_t v_val => Val_ok v_val v_t) v_t1 (LOCALS r_v_f) ->
+	Admin_instrs_ok v_S (upd_label (upd_local_return v_C (v_t1 ++ C_LOCALS v_C) ret) lab) [(AI_TRAP )] v_func_type.
+Proof.
+	intros.
+	destruct v_func_type.
+	rewrite <- admin_instrs_ok_eq.
+	apply AI_ok_trap.
+Qed.
+
+Lemma Step_read__load_num_val_preserves : forall v_S (r_v_f : frame) v_C (v_z : state) (v_i : nat) (v_t : valtype) (v_mo : memarg) v_c v_func_type v_t1 lab ret ,
+	Admin_instrs_ok v_S (upd_label (upd_local_return v_C (v_t1 ++ C_LOCALS v_C) ret) lab)[(AI_CONST I32 (fun_nat__u32 v_i : val_ I32));(AI_LOAD v_t None v_mo)] v_func_type ->
+	Module_instance_ok v_S (F_MODULE r_v_f) v_C  ->
+	v_z = mk_state v_S r_v_f ->
+	((fun_bytes_ v_t v_c) = (list_slice (BYTES (fun_mem v_z 0)) (v_i + (OFFSET v_mo)) ((fun_size v_t) / 8))) ->
+	Forall2 (fun v_t v_val => Val_ok v_val v_t) v_t1 (LOCALS r_v_f) ->
+	Admin_instrs_ok v_S (upd_label (upd_local_return v_C (v_t1 ++ C_LOCALS v_C) ret) lab) [(AI_CONST v_t v_c)] v_func_type.
+Proof.
+	move => v_S r_v_f v_C v_z v_i v_t v_mo v_c v_func_type v_t1 lab ret HType HMinst HState H HValOK.
+	destruct v_func_type as [ts1 ts2].
+	apply_composition_typing_and_single HType.
+	apply AI_const_typing in H4_comp0.
+	rewrite <- admin_instrs_ok_eq.
+	rewrite <- admin_instrs_ok_eq in H4_comp.
+Admitted. (*
+	apply Load_typing in H4_comp; destruct H4_comp as [ts [v_n [v_sx [v_inn [v_mt [? [? [? [? [? [? [? [??]]]]]]]]]]]]].
+	subst.
+	repeat rewrite -> app_assoc in H0; apply split_append_last in H0; destruct H0.
+	subst.
+	repeat rewrite -> app_assoc.
+	apply admin_instr_weakening_empty_1.
+	eapply (AI_ok_instr v_S _ (CONST v_t v_c) (mk_functype [] [v_t])).
+	apply const.
+Qed. *)
+
+(*
+Lemma Step_read__load_pack_trap_preserves : forall v_S (r_v_f : frame) v_C (v_z : state) (v_i : nat) (v_valtype : valtype) (v_n : n) (v_sx : sx) (v_mo : memarg) v_func_type v_t1 lab ret ,
+	Admin_instrs_ok v_S (upd_label (upd_local_return v_C (v_t1 ++ C_LOCALS v_C) ret) lab)[(AI_CONST I32 (fun_nat__u32 v_i));(AI_LOAD v_valtype (Some (op__ INN_I32 (mk_sz v_n) v_sx)) v_mo)] v_func_type ->
+	Module_instance_ok v_S (F_MODULE r_v_f) v_C  ->
+	v_z = mk_state v_S r_v_f ->
+	(((v_i + (OFFSET v_mo)) + (v_n / 8)) > (List.length (BYTES (fun_mem v_z 0))))%coq_nat ->
+	Forall2 (fun v_t v_val => Val_ok v_val v_t) v_t1 (LOCALS r_v_f) ->
+	Admin_instrs_ok v_S (upd_label (upd_local_return v_C (v_t1 ++ C_LOCALS v_C) ret) lab) [(AI_TRAP )] v_func_type.
+Proof.
+	intros.
+	destruct v_func_type.
+	rewrite <- admin_instrs_ok_eq.
+	apply AI_ok_trap.
+Qed.
+
+Lemma Step_read__load_pack_val_preserves : forall v_S (r_v_f : frame) v_C (v_z : state) (v_i : nat) (v_inn : inn) (v_n : n) (v_sx : sx) (v_mo : memarg) (v_c : iN 32) v_func_type v_t1 lab ret ,
+	Admin_instrs_ok v_S (upd_label (upd_local_return v_C (v_t1 ++ C_LOCALS v_C) ret) lab)[(AI_CONST I32 (v_i : val_));(AI_LOAD (valtype__INN v_inn) (Some ((packsize__ v_n), v_sx)) v_mo)] v_func_type ->
+	Module_instance_ok v_S (F_MODULE r_v_f) v_C  ->
+	v_z = mk_state v_S r_v_f ->
+	((fun_ibytes v_n v_c) = (list_slice (BYTES (fun_mem v_z 0)) (v_i + (OFFSET v_mo)) (v_n / 8))) ->
+	Forall2 (fun v_t v_val => Val_ok v_val v_t) v_t1 (LOCALS r_v_f) ->
+	Admin_instrs_ok v_S (upd_label (upd_local_return v_C (v_t1 ++ C_LOCALS v_C) ret) lab) [(AI_CONST (valtype__INN v_inn) (fun_ext v_n (fun_size (valtype__INN v_inn)) v_sx v_c))] v_func_type.
+Proof.
+	move => v_S r_v_f v_C v_z v_i v_inn v_n v_sx v_mo v_c v_func_type v_t1 lab ret HType HMinst HState H HValOK.
+	destruct v_func_type as [ts1 ts2].
+	apply_composition_typing_and_single HType.
+	apply AI_const_typing in H4_comp0.
+	rewrite <- admin_instrs_ok_eq.
+	rewrite <- admin_instrs_ok_eq in H4_comp.
+	apply Load_typing in H4_comp; destruct H4_comp as [ts [v_n' [v_sx' [v_inn' [v_mt [? [? [? [? [? [? [? [? ?]]]]]]]]]]]]].
+	subst.
+	repeat rewrite -> app_assoc in H0; apply split_append_last in H0; destruct H0.
+	subst.
+	repeat rewrite -> app_assoc.
+	apply admin_instr_weakening_empty_1.
+	eapply (AI_ok_instr v_S _ (CONST (valtype__INN v_inn) ((fun_ext v_n (fun_size (valtype__INN v_inn)) v_sx v_c))) (mk_functype [] [(valtype__INN v_inn)])).
+	apply const.
+Qed. *)
+
+Lemma Step_read__memory_size_preserves : forall v_S (r_v_f : frame) v_C (v_z : state) (v_n : n) v_func_type v_t1 lab ret ,
+	Admin_instrs_ok v_S (upd_label (upd_local_return v_C (v_t1 ++ C_LOCALS v_C) ret) lab)[(AI_MEMORY_SIZE )] v_func_type ->
+	Module_instance_ok v_S (F_MODULE r_v_f) v_C  ->
+	v_z = mk_state v_S r_v_f ->
+	(((v_n * 64) * (fun_Ki )) = (List.length (BYTES (fun_mem v_z 0)))) ->
+	Forall2 (fun v_t v_val => Val_ok v_val v_t) v_t1 (LOCALS r_v_f) ->
+	Admin_instrs_ok v_S (upd_label (upd_local_return v_C (v_t1 ++ C_LOCALS v_C) ret) lab) [(AI_CONST I32 (fun_nat__u32 v_n : val_ I32))] v_func_type.
+Proof.
+	move => v_S r_v_f v_C v_z v_n v_func_type v_t1 lab ret HType HMinst HState HLength HValOK.
+	destruct v_func_type as [ts1 ts2].
+	rewrite <- admin_instrs_ok_eq.
+	rewrite <- admin_instrs_ok_eq in HType.
+	apply Memory_size_typing in HType; destruct HType as [v_mt [? [? ?]]].
+	subst.
+	apply admin_instr_weakening_empty_1.
+	eapply (AI_ok_instr v_S _ (CONST (I32) (fun_nat__u32 v_n)) (mk_functype [] [(I32)])).
+	apply const.
+Qed.
+
+Lemma func_extension_same: forall f,
+	Forall2 (fun v s => Func_extension v s) f f.
+Proof.
+	move => f.
+	induction f => //.
+	apply Forall2_cons_iff. split.
+	- apply mk_Func_extension.
+	- apply IHf.
+Qed.
+
+Lemma table_extension_same: forall t,
+	Forall2 (fun v s => Table_extension v s) t t.
+Proof.
+	move => t.
+	induction t => //.
+	apply Forall2_cons_iff. split.
+	- destruct a as [type refs]. destruct type.
+	  destruct v__.
+	  apply mk_Table_extension => //.
+	- apply IHt.
+Qed.
+
+Lemma mem_extension_same: forall m,
+	Forall2 (fun v s => Mem_extension v s) m m.
+Proof.
+	move => m.
+	induction m => //.
+	apply Forall2_cons_iff. split.
+	- destruct a as [type bytes]. destruct type.
+	  destruct v__.
+	  apply mk_Mem_extension => //.
+	- apply IHm.
+Qed.
+
+Lemma global_extension_same: forall s g v_globaltype,
+	Forall2
+	(fun (v_globalinst : globalinst) (v_globaltype : globaltype) => Global_instance_ok s v_globalinst v_globaltype) g v_globaltype ->
+	Forall2 (fun v s => Global_extension v s) g g.
+Admitted.
+(* Proof.
+	move => s g v_globaltype HGlobalInstOk.
+	generalize dependent v_globaltype.
+	induction g => //; move => v_globaltype HGlobalInstOk.
+	apply Forall2_cons_iff. split.
+	-
+		apply Forall2_length in HGlobalInstOk as ?. 
+		destruct v_globaltype => //=.
+		inversion HGlobalInstOk.
+		inversion H3; decomp; subst.
+		inversion H11; subst.
+		apply Global_extension__. right => //.
+	- destruct v_globaltype; inversion HGlobalInstOk. eapply IHg; eauto. 
+Qed. *)
+
+Lemma store_extension_same: forall s,
+	Store_ok s ->
+    Store_extension s s.
+Admitted.
+(* Proof.
+  move => s HST. 
+  inversion HST; decomp.
+  apply (Store_extension__ s s (FUNCS s) (TABLES s) (MEMS s) (GLOBALS s) (FUNCS s) [] (TABLES s) [] (MEMS s) [] (GLOBALS s) []).
+  repeat (split => //; try rewrite -> app_nil_r).
+  + by apply func_extension_same.
+  + by apply table_extension_same.
+  + by apply mem_extension_same.
+  + subst. eapply global_extension_same; eauto.
+Qed. *)
+
+Lemma config_same: forall s f ais s' f' ais',
+	(mk_config (mk_state s f) ais) = (mk_config (mk_state s' f') ais') ->
+	s = s' /\ f = f' /\ ais = ais'.
+Proof.
+	move => s f ais s' f' ais' H.
+	injection H as H1 => //=.
+Qed.
+
+Lemma config_same2: forall s f ais s' f' ais',
+	s = s' /\ f = f' /\ ais = ais' ->
+ 	(mk_config (mk_state s f) ais) = (mk_config (mk_state s' f') ais').
+Proof.
+	move => s f ais s' f' ais' [? [? ?]].
+	f_equal => //=. f_equal => //=.
+Qed.
+
+Lemma Forall2_global: forall v_S v_globaltype v_idx v_valtype v_val_0 v_val_,
+	Forall2
+	(fun (v_globalinst : globalinst) (v_globaltype : globaltype) => Global_instance_ok v_S v_globalinst v_globaltype) (GLOBALS v_S) v_globaltype -> 
+	(v_idx < length (GLOBALS v_S))%coq_nat ->
+	lookup_total (GLOBALS v_S) v_idx = 
+	{| GLOB_TYPE := mk_globaltype (Some MUT) v_valtype; VALUE := VAL_CONST v_valtype v_val_0 |} ->
+	Forall2 (fun v s => Global_extension v s) (GLOBALS v_S) (list_update_func (GLOBALS v_S) v_idx 
+		(fun g => g <| VALUE := (VAL_CONST v_valtype v_val_) |> )).
+Admitted.
+(* Proof.
+	move => v_S v_globaltype v_idx v_val0 v_valtype v_val_.
+	destruct v_S as [funcs globals tables mems]; simpl.
+	move: v_idx v_globaltype.
+	induction globals; move => v_idx v_globaltype HGlobalInstOk H H2 => //=.
+	destruct v_idx => //=.
+	
+	apply Forall2_cons_iff. unfold lookup_total in H2; simpl in H2; subst. split.
+	- unfold set. simpl. apply Global_extension__. left => //.
+		destruct v_globaltype; inversion HGlobalInstOk.
+		eapply global_extension_same; eauto. 
+	- apply Forall2_cons. 
+		-
+			apply Forall2_length in HGlobalInstOk as ?. 
+			destruct v_globaltype => //=.
+			inversion HGlobalInstOk.
+			inversion H5; decomp; subst.
+			inversion H13; subst.
+			apply Global_extension__. right => //.
+		- unfold lookup_total in H2. simpl in H2. 
+			destruct v_globaltype; inversion HGlobalInstOk.
+			eapply IHglobals => //=.
+			- 
+				apply Forall2_length in H6.
+				apply Forall2_forall2; split => //=.
+				apply H6.
+				move => x0 y0 Hin.
+				inversion HGlobalInstOk; subst.
+				apply Forall2_forall2 in H12; destruct H12.
+				apply H1 in Hin.
+				inversion Hin; decomp; subst.
+				inversion H11.
+				eapply Global_instance_ok__; repeat split => //=.
+			- simpl in H. apply Nat.succ_lt_mono in H. apply H.
+Qed. *)
+
+Lemma update_global_unchagned: forall v_S v_S' v_f v_x v_valtype v_val_,
+	v_S' =
+	v_S <| GLOBALS :=
+	list_update_func (GLOBALS v_S)
+	(lookup_total (MODULE_GLOBALS (F_MODULE v_f)) v_x)
+	[eta set VALUE (fun=> VAL_CONST v_valtype v_val_)] |> ->
+	FUNCS v_S = FUNCS v_S' /\
+	TABLES v_S = TABLES v_S' /\
+	length (GLOBALS v_S) = length (GLOBALS v_S') /\
+	MEMS v_S = MEMS v_S'.
+Proof. 
+	move => v_S v_S' v_f v_x v_valtype v_val' H.
+	destruct v_S'. unfold set in H. simpl in *.
+	injection H as ?; subst; repeat split => //=.
+	by erewrite <- list_update_length_func.
+Qed.
+
+Lemma update_mem_unchagned_func: forall v_S v_S' func v_idx,
+	v_S' = v_S <| MEMS := list_update_func (MEMS v_S) v_idx func |> ->
+	FUNCS v_S = FUNCS v_S' /\
+	TABLES v_S = TABLES v_S' /\
+	length (MEMS v_S) = length (MEMS v_S') /\
+	GLOBALS v_S = GLOBALS v_S'.
+Proof.
+	move => v_S v_S' func v_idx H.
+	destruct v_S'. unfold set in H. simpl in *.
+	injection H as ?; subst; repeat split => //=.
+	by erewrite <- list_update_length_func.
+Qed.
+
+Lemma update_mem_unchagned: forall v_S v_S' func v_idx,
+	v_S' = v_S <| MEMS := list_update (MEMS v_S) v_idx func |> ->
+	FUNCS v_S = FUNCS v_S' /\
+	TABLES v_S = TABLES v_S' /\
+	length (MEMS v_S) = length (MEMS v_S') /\
+	GLOBALS v_S = GLOBALS v_S'.
+Proof.
+	move => v_S v_S' func v_idx H.
+	destruct v_S'. unfold set in H. simpl in *.
+	injection H as ?; subst; repeat split => //=.
+	by erewrite <- list_update_length.
+Qed.
+
+Lemma func_agree_extension: forall v_S v_S' v_funcaddr v_funcinst_1' v_funcinst_2 v_functype,
+	Externaddrs_ok v_S (EXTVAL_FUNC v_funcaddr) (EXT_FUNC v_functype) ->
+	length (FUNCS v_S) = length v_funcinst_1' ->
+	FUNCS v_S' = (v_funcinst_1' ++ v_funcinst_2)%list -> 
+    Forall2 (fun v s => Func_extension v s) (FUNCS v_S) v_funcinst_1' ->
+    Externaddrs_ok v_S' (EXTVAL_FUNC v_funcaddr) (EXT_FUNC v_functype).
+Admitted.
+(* Proof.
+	move => v_S v_S' v_funcaddr v_funcinst_1' v_funcinst_2 v_functype HOk HLength HApp Hext.
+	inversion HOk; destruct H2; subst.
+	apply Forall2_nth in Hext; destruct Hext.
+	apply (H0 _ default_val default_val) in H2 as H2'.
+	unfold lookup_total in H3.
+	apply (Externaddrs_ok__func _ _ _ v_minst v_code_func).
+	apply (length_app_lt) with (l':=(FUNCS v_S')) (l2':= v_funcinst_2) in HLength => //=.
+	split. 
+	- apply (Nat.lt_le_trans _ _ _ H2 HLength).
+	- unfold lookup_total.
+		rewrite H in H2.
+		apply app_nth1 with (l' := v_funcinst_2) (d := default_val) in H2.
+		rewrite <- HApp in H2.
+		destruct default_val.
+		inversion H2'.
+		rewrite H2. 
+		rewrite <- H5.
+		apply H3.
+Qed. *)
+
+Lemma table_agree_extension: forall v_S v_S' v_tableaddr v_tableinst_1' v_tableinst_2 v_tabletype,
+    Externaddrs_ok v_S (EXTVAL_TABLE v_tableaddr) (EXT_TABLE v_tabletype) ->
+	length (TABLES v_S) = length v_tableinst_1' ->
+	TABLES v_S' = (v_tableinst_1' ++ v_tableinst_2) -> 
+	Forall2 (fun v s => Table_extension v s) (TABLES v_S) v_tableinst_1' ->
+    Externaddrs_ok v_S' (EXTVAL_TABLE v_tableaddr) (EXT_TABLE v_tabletype).
+Admitted.
+(* Proof.
+	move => v_S v_S' v_tableaddr v_tableinst_1' v_tableinst_2 v_tabletype HOk HLength HApp Hext.
+	inversion HOk; destruct H2; subst; destruct H3.
+	apply Forall2_lookup in Hext; destruct Hext.
+	apply H3 in H2 as H2'.
+	inversion H2'. 
+	eapply Externaddrs_ok__table.
+	apply (length_app_lt) with (l':=(TABLES v_S')) (l2':= v_tableinst_2) in HLength => //=.
+	split.
+	- apply (Nat.lt_le_trans _ _ _ H2 HLength).
+	-  
+		rewrite H1 in H2.
+		apply lookup_app with (l' := v_tableinst_2) in H2.
+		rewrite <- HApp in H2.
+		rewrite <- H2.
+		rewrite <- H5. split => //=.
+		rewrite <- H4 in H.
+		injection H as ?.
+		inversion H0. inversion H8. destruct H11.
+		subst.
+		injection H12 as ?.
+		apply Tabletype_sub__.
+		apply Limits_sub__.
+		subst.
+		unfold ge in H11. split.
+		unfold ge.
+		eapply Nat.le_trans; eauto.
+		apply H14.
+Qed. *)
+
+Lemma global_agree_extension: forall v_S v_S' v_globaladdr v_globalinst_1' v_globalinst_2 v_globaltype,
+    Externaddrs_ok v_S (EXTVAL_GLOBAL v_globaladdr) (EXT_GLOBAL v_globaltype) ->
+	length (GLOBALS v_S) = length v_globalinst_1' ->
+	GLOBALS v_S' = (v_globalinst_1' ++ v_globalinst_2) -> 
+	Forall2 (fun v s => Global_extension v s) (GLOBALS v_S) v_globalinst_1' ->
+    Externaddrs_ok v_S' (EXTVAL_GLOBAL v_globaladdr) (EXT_GLOBAL v_globaltype).
+Admitted.
+(* Proof.
+	move => v_S v_S' v_globaladdr v_globalinst_1' v_globalinst_2 v_globaltype HOk HLength HApp Hext.
+	inversion HOk; destruct H2; subst.
+	apply Forall2_lookup in Hext; destruct Hext.
+	apply H0 in H2 as H2'.
+	inversion H2'.
+	eapply Externaddrs_ok__global with (v_val_ := v_c2).
+	apply (length_app_lt) with (l':=(GLOBALS v_S')) (l2':= v_globalinst_2) in HLength => //=.
+	split.
+	- apply (Nat.lt_le_trans _ _ _ H2 HLength).
+	- 
+		rewrite H in H2.
+		apply lookup_app with (l' := v_globalinst_2) in H2.
+		rewrite <- HApp in H2.
+		rewrite <- H2.
+		rewrite <- H1 in H3.
+		injection H3 as ?.
+		subst => //=.
+Qed. *)
+
+Lemma mem_agree_extension: forall v_S v_S' v_memaddr v_meminst_1' v_meminst_2 v_memtype,
+    Externaddrs_ok v_S (EXTVAL_MEM v_memaddr) (EXT_MEM v_memtype) ->
+	length (MEMS v_S) = length v_meminst_1' ->
+	MEMS v_S' = (v_meminst_1' ++ v_meminst_2) -> 
+	Forall2 (fun v s => Mem_extension v s) (MEMS v_S) v_meminst_1' ->
+    Externaddrs_ok v_S' (EXTVAL_MEM v_memaddr) (EXT_MEM v_memtype).
+Admitted.
+(* Proof.
+	move => v_S v_S' v_memaddr v_meminst_1' v_meminst_2 v_memtype HOk HLength HApp Hext.
+	inversion HOk; destruct H2; subst; destruct H3 as [? ?].
+	apply Forall2_lookup in Hext; destruct Hext.
+	apply H3 in H2 as H2'.
+	inversion H2'. 
+	eapply Externaddrs_ok__mem.
+	apply (length_app_lt) with (l':=(MEMS v_S')) (l2':= v_meminst_2) in HLength => //=.
+	split.
+	- apply (Nat.lt_le_trans _ _ _ H2 HLength).
+	-  
+		rewrite H1 in H2.
+		apply lookup_app with (l' := v_meminst_2) in H2.
+		rewrite <- HApp in H2.
+		rewrite <- H2.
+		rewrite <- H5. repeat split => //=. 
+		rewrite <- H4 in H.
+		injection H as ?.
+		inversion H0. inversion H8. destruct H11.
+		subst.
+		injection H12 as ?.
+		apply Limits_sub__.
+		subst.
+		unfold ge in H11. split.
+		unfold ge.
+		eapply Nat.le_trans; eauto.
+		apply H14.
+Qed. *)
+
+Lemma func_extension_C: forall v_S v_S' v_funcaddrs v_funcinst_1' v_funcinst_2 tcf,
+    Forall2 (fun v s => Externaddrs_ok v_S (EXTVAL_FUNC v) (EXT_FUNC s)) v_funcaddrs tcf ->
+	length (FUNCS v_S) = length v_funcinst_1' ->
+	FUNCS v_S' = (v_funcinst_1' ++ v_funcinst_2)%list -> 
+	Forall2 (fun v s => Func_extension v s) (FUNCS v_S) v_funcinst_1' ->
+    Forall2 (fun v s => Externaddrs_ok v_S' (EXTVAL_FUNC v) (EXT_FUNC s)) v_funcaddrs tcf.
+Proof.
+	move => v_S v_S' v_funcaddrs v_funcinst_1' v_funcinst_2.
+	move: v_S v_S'.
+	induction v_funcaddrs;
+	move => v_S v_S' tcf HOk Hlength HApp Hext => //=; destruct tcf => //=; simpl in HOk; try (apply Forall2_length in HOk; discriminate).
+	subst.
+	apply Forall2_cons_iff. split.
+	- inversion HOk; subst. apply (func_agree_extension v_S) with (v_funcinst_1' := v_funcinst_1') (v_funcinst_2 := v_funcinst_2) => //.
+	- eapply IHv_funcaddrs. inversion HOk. apply H4. apply Hlength. apply HApp. apply Hext.
+Qed. 	
+
+Lemma table_extension_C: forall v_S v_S' v_tableaddrs v_tableinst_1' v_tableinst_2 tcf,
+    Forall2 (fun v s => Externaddrs_ok v_S (EXTVAL_TABLE v) (EXT_TABLE s)) v_tableaddrs tcf ->
+	length (TABLES v_S) = length v_tableinst_1' ->
+	TABLES v_S' = (v_tableinst_1' ++ v_tableinst_2)%list -> 
+	Forall2 (fun v s => Table_extension v s) (TABLES v_S) v_tableinst_1' ->
+    Forall2 (fun v s => Externaddrs_ok v_S' (EXTVAL_TABLE v) (EXT_TABLE s)) v_tableaddrs tcf.
+Proof.
+	move => v_S v_S' v_tableaddrs v_tableinst_1' v_tableinst_2.
+	move: v_S v_S'.
+	induction v_tableaddrs;
+	move => v_S v_S' tcf HOk Hlength HApp Hext => //=; destruct tcf => //=; simpl in HOk; try (apply Forall2_length in HOk; discriminate).
+	subst.
+	apply Forall2_cons_iff. split.
+	- inversion HOk; subst. apply (table_agree_extension v_S) with (v_tableinst_1' := v_tableinst_1') (v_tableinst_2 := v_tableinst_2) => //.
+	- eapply IHv_tableaddrs. inversion HOk. apply H4. apply Hlength. apply HApp. apply Hext.
+Qed. 	
+
+Lemma global_extension_C: forall v_S v_S' v_globaladdrs v_globalinst_1' v_globalinst_2 tcf,
+    Forall2 (fun v s => Externaddrs_ok v_S (EXTVAL_GLOBAL v) (EXT_GLOBAL s)) v_globaladdrs tcf ->
+	length (GLOBALS v_S) = length v_globalinst_1' ->
+	GLOBALS v_S' = (v_globalinst_1' ++ v_globalinst_2)%list -> 
+	Forall2 (fun v s => Global_extension v s) (GLOBALS v_S) v_globalinst_1' ->
+    Forall2 (fun v s => Externaddrs_ok v_S' (EXTVAL_GLOBAL v) (EXT_GLOBAL s)) v_globaladdrs tcf.
+Proof.
+	move => v_S v_S' v_globaladdrs v_globalinst_1' v_globalinst_2.
+	move: v_S v_S'.
+	induction v_globaladdrs;
+	move => v_S v_S' tcf HOk Hlength HApp Hext => //=; destruct tcf => //=; simpl in HOk; try (apply Forall2_length in HOk; discriminate).
+	subst.
+	apply Forall2_cons_iff. split.
+	- inversion HOk; subst. apply (global_agree_extension v_S) with (v_globalinst_1' := v_globalinst_1') (v_globalinst_2 := v_globalinst_2) => //.
+	- eapply IHv_globaladdrs. inversion HOk. apply H4. apply Hlength. apply HApp. apply Hext.
+Qed.
+
+
+Lemma mem_extension_C: forall v_S v_S' v_memaddrs v_meminst_1' v_meminst_2 tcf,
+	Forall2 (fun v s => Externaddrs_ok v_S (EXTVAL_MEM v) (EXT_MEM s)) v_memaddrs tcf ->
+	length (MEMS v_S) = length v_meminst_1' ->
+	MEMS v_S' = (v_meminst_1' ++ v_meminst_2)%list -> 
+	Forall2 (fun v s => Mem_extension v s) (MEMS v_S) v_meminst_1' ->
+    Forall2 (fun v s => Externaddrs_ok v_S' (EXTVAL_MEM v) (EXT_MEM s)) v_memaddrs tcf.
+Proof.
+	move => v_S v_S' v_memaddrs v_meminst_1' v_meminst_2.
+	move: v_S v_S'.
+	induction v_memaddrs;
+	move => v_S v_S' tcf HOk Hlength HApp Hext => //=; destruct tcf => //=; simpl in HOk; try (apply Forall2_length in HOk; discriminate).
+	subst.
+	apply Forall2_cons_iff. split.
+	- inversion HOk; subst. apply (mem_agree_extension v_S) with (v_meminst_1' := v_meminst_1') (v_meminst_2 := v_meminst_2) => //.
+	- eapply IHv_memaddrs. inversion HOk. apply H4. apply Hlength. apply HApp. apply Hext.
+Qed.
+
+Lemma ext_extension_C: forall v_S v_S' v_exportinst,
+	Store_extension v_S v_S' ->
+	Forall (Export_instance_ok v_S) v_exportinst -> 
+	Forall (Export_instance_ok v_S') v_exportinst.
+Proof.
+	move => v_S v_S' v_exportinst.
+	move: v_S v_S'.
+	induction v_exportinst;
+	move => v_S v_S' Hext HOk => //=.
+	subst. inversion HOk. 
+	apply Forall_cons_iff. split.
+	-	inversion H1.
+		subst.
+		eapply mk_Export_instance_ok with (v_ext := v_ext).
+		inversion Hext; decomp. 
+		inversion H3; subst; destruct H20.
+		- inversion H6.
+		- inversion H7.
+		- inversion H8.
+		- inversion H9.
+	- eapply IHv_exportinst; eauto.
+Qed.
+
+Lemma module_inst_typing_extension: forall v_S v_S' v_i v_C,
+    Store_extension v_S v_S' ->
+    Module_instance_ok v_S v_i v_C ->
+    Module_instance_ok v_S' v_i v_C.
+Admitted.
+(* Proof.
+	move => v_S v_S' v_i v_C HStoreExtension HMIT.
+	inversion HStoreExtension. 
+	inversion HMIT; decomp.
+	subst.
+	apply Module_instance_ok__; repeat split => //=.
+	- eapply func_extension_C; eauto.
+	- eapply table_extension_C; eauto.
+	- eapply global_extension_C ; eauto.
+	- eapply mem_extension_C; eauto.
+	- eapply ext_extension_C; eauto.
+Qed. *)
+
+Lemma global_instance_fine: forall s s' v_globaltype v_f v_x v_valtype v_val_,
+    Forall2 (fun v vt => Global_instance_ok s v vt) (GLOBALS s) v_globaltype ->
+	Forall2 (fun g g' => Global_extension g g') (GLOBALS s) (GLOBALS s') ->
+	(FUNCS s = FUNCS s') ->
+	(TABLES s = TABLES s') ->
+	(MEMS s = MEMS s') ->
+	(GLOBALS s') = list_update_func (GLOBALS s)
+	(lookup_total (MODULE_GLOBALS (F_MODULE v_f)) v_x)
+	[eta set VALUE (fun=> VAL_CONST v_valtype v_val_)] -> 
+	Forall2 (fun v vt => Global_instance_ok s' v vt) (GLOBALS s) v_globaltype.
+Admitted.
+(* Proof.
+	move => s s' v_globaltype v_f v_x v_valtype v_val_ HGlobalInstOk HGlobExt HFEq HTab HMems HGlob.
+
+	destruct s as [funcs1 globals1 tables1 mems1]. destruct s' as [funcs2 globals2 tables2 mems2].
+	simpl in *. subst funcs1. subst tables1. subst mems1.
+	generalize dependent v_globaltype.
+	induction globals1; move => v_globaltype HGlobalInstOk; apply Forall2_length in HGlobalInstOk as H'.
+	- symmetry in H'. 
+		apply List.length_zero_iff_nil in H'. 
+		subst. 
+		apply Forall2_nil.
+	- destruct v_globaltype => //=.
+		apply Forall2_cons_iff. split.
+		- inversion HGlobalInstOk; subst.
+			inversion H2. destruct H as [? [? ?]].
+			inversion H6; subst.
+			eapply Global_instance_ok__; eauto.
+		- apply Forall2_forall2; split.
+			- simpl in H'. by injection H' as ?.
+			- move => x y Hin.
+				inversion HGlobalInstOk.
+				subst.
+				apply Forall2_forall2 in H4; destruct H4.
+				apply H0 in Hin.
+				inversion Hin; subst. destruct H1 as [? [? ?]].
+				inversion H4; subst.
+				eapply Global_instance_ok__; eauto.
+Qed. *)
+
+Lemma store_global_extension_store_typed: forall s s' v_f v_C v_valtype v_val_ v_x v_mut v_valtype0 v_val_0,
+    Store_ok s ->
+    Store_extension s s' ->
+	Module_instance_ok s (F_MODULE v_f) v_C ->
+	Module_instance_ok s' (F_MODULE v_f) v_C ->
+	(GLOBALS s') = list_update_func (GLOBALS s)
+	(lookup_total (MODULE_GLOBALS (F_MODULE v_f)) v_x)
+	[eta set VALUE (fun=> VAL_CONST v_valtype v_val_)] ->
+	lookup_total (GLOBALS s) (lookup_total (MODULE_GLOBALS (F_MODULE v_f)) v_x) =
+	{|
+	GLOB_TYPE := mk_globaltype v_mut v_valtype0;
+	VALUE := VAL_CONST v_valtype0 v_val_0
+	|} ->
+	Datatypes.length (GLOBALS s) = Datatypes.length (GLOBALS s') ->
+    (FUNCS s = FUNCS s') ->
+    (TABLES s = TABLES s') ->
+    (MEMS s = MEMS s') ->
+	((lookup_total (MODULE_GLOBALS (F_MODULE v_f)) v_x) < length (GLOBALS s))%coq_nat ->
+    Store_ok s'.
+Admitted.
+(* Proof.
+	move => s s' f C v_valtype v_val_ v_x v_mut v_valtype0 v_val_0 HSOK Hext HIT HITS' HUpdate HGlobInst HLGlobal HFeq HTeq HMeq HLength.
+	inversion HSOK; decomp.
+	inversion Hext; decomp; subst.
+	destruct s' as [funcs2 globals2 tables2 mems2].
+	apply f_equal with (f := fun t => List.length t) in HMeq as ?.
+	apply f_equal with (f := fun t => List.length t) in HTeq as ?.
+	apply f_equal with (f := fun t => List.length t) in HFeq as ?.
+	removeinst2 H22. 
+	removeinst2 H20.
+	removeinst2 H19.
+	removeinst2 H21. subst.
+	simpl in *.
+	eapply Store_ok__OK with (v_funcinst := v_funcinst) (v_functype := v_functype)
+		(v_tableinst := v_tableinst) (v_tabletype := v_tabletype)
+		(v_meminst := v_meminst) (v_memtype := v_memtype)
+		(v_globalinst := globals2) (v_globaltype := v_globaltype); subst; repeat split => //=.
+	- rewrite HLGlobal in H1 => //=. 
+	- f_equal => //=.
+	- apply Forall2_forall2; split => //=. move => x y HIn.
+		apply Forall2_forall2 in H5; destruct H5. apply H11 in HIn. inversion HIn; destruct H15 as [? [? ?]].
+		eapply Function_instance_ok__ with (v_C := v_C); repeat split => //=.
+		eapply module_inst_typing_extension; eauto.
+	- eapply Forall2_list_update_func; eauto.
+		- remember ({|
+				FUNCS := funcs2;
+				GLOBALS := v_globalinst;
+				TABLES := tables2;
+				MEMS := mems2
+			|}) as s.
+			assert (v_globalinst = (GLOBALS s)). {by subst. }
+			rewrite H11.
+			eapply global_instance_fine; subst; simpl; eauto.
+			apply Forall2_lookup in H26; destruct H26.
+			apply H15 in HLength as H''.
+			rewrite HGlobInst in H''.
+			inversion H''.
+			subst.
+			apply Forall2_lookup in H6; destruct H6.
+			apply H16 in HLength as H'''.
+			rewrite HGlobInst in H'''.
+			inversion H'''.
+			destruct H22 as [? [? ?]].
+			eapply Global_instance_ok__; repeat split => //=.
+			inversion H29. subst.
+			eapply lookup_list_update_func in H21; eauto; destruct H21 as [y ?].
+			unfold set in H18.
+			injection H18 as ?; subst.
+			apply Val_ok__.
+	- apply Forall2_forall2; split => //=. move => x y HIn.
+		apply Forall2_forall2 in H7; destruct H7. apply H11 in HIn. inversion HIn; decomp; subst.
+		eapply Table_instance_ok__; repeat split => //=; eauto.
+		apply Forall2_forall2; split => //=. move => x y HIn'. apply Forall2_forall2 in H21; destruct H21.
+		apply H17 in HIn'. apply Forall2_forall2 in HIn'; destruct HIn'.
+		apply Forall2_forall2; split => //=. move => x' y' HIn''.
+		apply H20 in HIn''. inversion HIn''; decomp; subst. eapply Externaddrs_ok__func; eauto.
+	- apply Forall2_forall2; split => //=. move => x y HIn.
+		apply Forall2_forall2 in H8; destruct H8. apply H11 in HIn. inversion HIn; decomp; subst. 
+		eapply Memory_instance_ok__; repeat split => //=; eauto.
+Qed. *)
+
+Lemma t_preservation_vs_type: forall s f ais s' f' ais' C C' v_t1 lab ret t1s t2s,
+    Step (mk_config (mk_state s f) ais) (mk_config (mk_state s' f') ais') ->
+    Store_ok s -> 
+	Store_ok s' ->
+    Module_instance_ok s (F_MODULE f) C ->
+    Module_instance_ok s' (F_MODULE f') C' ->
+	v_t1 = (C_LOCALS (upd_label (upd_local_return C (v_t1 ++ (C_LOCALS C)) ret) lab)) -> 
+	Forall2 (fun v_t v_val => Val_ok v_val v_t) v_t1 (LOCALS f) ->
+    Admin_instrs_ok s (upd_label (upd_local_return C (v_t1 ++ (C_LOCALS C)) ret) lab) ais (mk_functype t1s t2s) ->
+    Forall2 (fun v_t v_val0 => Val_ok v_val0 v_t) v_t1 (LOCALS f') 
+	/\ length v_t1 = length (LOCALS f').
+Admitted.
+(* Proof.
+	move => s f ais s' f' ais' C C' v_t1 
+		lab ret t1s t2s HReduce HStore HStore' HMInst HMInst' HValTypeEq HValOK HType.
+	remember (mk_config (mk_state s f) ais) as c1.
+	remember (mk_config (mk_state s' f') ais') as c2.
+	generalize dependent t2s. generalize dependent t1s.
+	generalize dependent lab. generalize dependent ais'. generalize dependent ais.
+	induction HReduce; try intros; try (induction v_z; subst); 
+	try (apply config_same in Heqc1; apply config_same in Heqc2; 
+		destruct Heqc1 as [Hbefore1 [Hbefore2 Hbefore3]]; 
+		destruct Heqc2 as [Hafter1 [Hafter2 Hafter3]]; split; subst => //; try apply Forall2_length in HValOK as ? => //).
+	- (* Label Context *)
+		injection Heqc1 as ?.
+		injection Heqc2 as ?; subst.
+		apply_composition_typing_single HType.
+		apply Label_typing in H4_comp; destruct H4_comp as [ts [ts2' [? [? [? ?]]]]]; subst.
+		rewrite upd_label_overwrite in H2; simpl in H2.
+		simpl in HValTypeEq.
+		eapply IHHReduce; eauto.
+	- (* Local Set *)
+		rewrite -> Forall2_Val_ok_is_same_as_map in HValOK; rewrite -> Forall2_Val_ok_is_same_as_map.
+		induction v_val.
+		apply_composition_typing_and_single HType.
+		apply AI_const_typing in  H4_comp0.
+		apply_composition_typing_single H4_comp.
+		apply Set_local_typing in H4_comp1; destruct H4_comp1 as [t [HLookup [H0' H1']]].
+		subst.
+		repeat rewrite -> app_assoc in H1_comp1; apply split_append_last in H1_comp1; destruct H1_comp1.
+		replace (C_LOCALS C) with ([::]: list valtype) in *; last by symmetry; eapply inst_t_context_local_empty; eauto.
+		rewrite -> cats0 in *.
+		simpl in H1'; simpl in H0. rewrite -> List.map_length in H1'. 
+		apply list_update_map with (f := typeof) (val := (VAL_CONST v_valtype v_val_)) in H1' as HUpdate.
+		rewrite HUpdate.
+		rewrite list_update_same_unchanged => //=; try rewrite List.map_length => //=.
+		simpl. by rewrite list_update_length.
+Qed. *)
+
+Lemma store_extension_reduce: forall s f ais s' f' ais' C tf loc lab ret,
+    Step (mk_config (mk_state s f) ais) (mk_config (mk_state s' f') ais') ->
+    Module_instance_ok s (F_MODULE f) C ->
+    Admin_instrs_ok s (upd_label (upd_local_return C loc ret) lab) ais tf ->
+    Store_ok s ->
+    Store_extension s s' /\ Store_ok s'.
+Admitted.
+(* Proof.
+	move => s f ais s' f' ais' C tf loc lab ret HReduce HIT HType HStore.
+	remember (mk_config (mk_state s f) ais) as c1.
+	remember (mk_config (mk_state s' f') ais') as c2.
+	generalize dependent C. generalize dependent tf.
+  	generalize dependent loc. generalize dependent lab. generalize dependent ret.
+	generalize dependent ais. generalize dependent ais'. 
+	generalize dependent f. generalize dependent f'.
+	induction HReduce; try move => f' f ais' Heqc2 ais Heqc1 ret lab loc tf C HIT HType HST; try intros; destruct tf;
+	try (destruct v_z; 
+	apply config_same in Heqc1; apply config_same in Heqc2; 
+	destruct Heqc1; destruct Heqc2;
+	subst; try (split => //; eapply store_extension_same; eauto)).
+	- (* Label Context *) 
+		injection Heqc1 as H1.
+		injection Heqc2 as H2.
+		rewrite <- H in HType.
+		apply_composition_typing_single HType.
+		apply Label_typing in H4_comp; destruct H4_comp as [ts [ts2' [? [? [? ?]]]]]; subst.
+		rewrite upd_label_overwrite in H6; simpl in H6.
+		eapply IHHReduce; eauto.
+	- (* Label Frame *)
+		injection Heqc1 as H1.
+		injection Heqc2 as H2.
+		rewrite <- H0 in HType.
+		apply_composition_typing_single HType.
+		apply Frame_typing in H4_comp. destruct H4_comp as [ts [? [? ?]]].
+		inversion H6. destruct H8.
+		inversion H8. destruct H15 as [? [? ?]]; subst.
+		simpl in H14.
+		rewrite <- upd_return_is_same_as_append in H14; simpl in H14.
+		rewrite <- upd_local_is_same_as_append in H14; simpl in H14.
+		rewrite -> _append_option_none_left in H14.
+		apply upd_label_unchanged_typing in H14.
+		eapply IHHReduce; eauto.
+	- (* Global Set *) 
+		destruct H2; destruct H0; subst.
+		apply_composition_typing_and_single HType.
+		destruct v_val.
+		apply AI_const_typing in H4_comp0.
+		rewrite <- admin_instrs_ok_eq in H4_comp.
+		apply Set_global_typing in H4_comp; destruct H4_comp as [t [? [?  ?]]].
+		remember  (s <| GLOBALS :=
+			list_update_func (GLOBALS s)
+		  	(lookup_total (MODULE_GLOBALS (F_MODULE f)) v_x)
+		  	[eta set VALUE (fun=> VAL_CONST v_valtype v_val_)] |>) as s'.
+		assert (Store_extension s s'). 
+		{
+			eapply Store_extension__ with (v_globalinst_1 := (GLOBALS s)) (v_globalinst_1' := (GLOBALS s')) (v_globalinst_2 := []); 
+			repeat split => //=; subst; simpl => //=; try rewrite <- app_right_nil => //=.
+			- by rewrite list_update_length_func.
+			- by eapply func_extension_same.
+			- by eapply table_extension_same.
+			- by eapply mem_extension_same.
+			- inversion HIT; decomp; subst; simpl in *. 
+				remember ((lookup_total v_globaladdr v_x)) as v.
+				apply Forall2_lookup2 in H12; destruct H12.
+				apply H5 in H1. inversion H1; destruct H17.
+				repeat rewrite -> app_assoc in H0; apply split_append_last in H0; destruct H0.
+				subst.
+				rewrite H in H16. injection H16 as ?; subst.
+				inversion HStore; decomp; subst. 
+				eapply Forall2_global; eauto. 
+		}
+		split => //=.
+		eapply module_inst_typing_extension with (v_S' := s') in HIT as HITS'; eauto.
+		apply update_global_unchagned in Heqs' as ?.
+		destruct H3 as [? [? [??]]].
+		inversion HIT; decomp; subst.
+		simpl in *.
+		inversion HStore; decomp; subst; simpl in *.
+		apply Forall2_lookup2 in H17; destruct H17.
+		apply H17 in H1.
+		inversion H1. destruct H29. simpl in *.
+		destruct H30.
+		eapply store_global_extension_store_typed; eauto.
+		- unfold set. simpl. reflexivity.
+		- rewrite <- H7. simpl. apply H30.
+		- simpl. by rewrite <- H7.
+	- (* Store Num Val *)
+		destruct H3; destruct H1; subst.
+		apply_composition_typing_and_single HType.
+		apply_composition_typing_and_single H4_comp.
+		apply AI_const_typing in H4_comp0.
+		apply AI_const_typing in H4_comp.
+		rewrite <- admin_instrs_ok_eq in H4_comp1.
+		apply Store_typing in H4_comp1; destruct H4_comp1 as [v_n [v_mt [v_inn [? [? [? [? [? ?]]]]]]]].
+		subst.
+		remember ((s <| MEMS :=
+		list_update_func (MEMS s)
+		  (lookup_total (MODULE_MEMS (F_MODULE f)) 0)
+		  (λ v_1 : meminst,
+			 v_1 <| BYTES :=
+			 list_slice_update (BYTES v_1) (v_i + OFFSET v_mo)%coq_nat
+			   (fun_size v_t / 8) (fun_bytes_ v_t v_c) |>) |>)) as s'.
+		assert (Store_extension s s').
+		{
+			eapply Store_extension__ with (v_meminst_1 := (MEMS s)) (v_meminst_1' := (MEMS s')) (v_meminst_2 := []);
+			repeat split; subst; simpl; try rewrite <- app_right_nil => //=.
+			- by rewrite list_update_length_func.
+			- by eapply func_extension_same.
+			- by eapply table_extension_same.
+			- (* Mem extension *)
+				inversion HIT; decomp; subst; simpl in *.
+				apply Forall2_lookup2 in H15; destruct H15. apply H7 in H0.
+				inversion H0; decomp; subst.
+				inversion HStore; decomp; subst; simpl in *.
+				eapply Forall2_list_update_func2; eauto.
+				- by apply mem_extension_same.
+				- unfold set; simpl. destruct v_mt'. apply mk_Mem_extension => //=.
+			- inversion HStore; decomp; subst; simpl in *.
+				eapply global_extension_same; eauto.
+		}
+		split => //=.
+		eapply update_mem_unchagned_func in Heqs' as ?; decomp.
+		subst; simpl in *.
+		destruct s. simpl in *.
+		inversion HStore; decomp; subst. 
+		injection H14 as ?; subst.
+		eapply Store_ok__OK; repeat split; simpl; eauto.
+		- erewrite list_update_length_func; eauto.
+		- apply Forall2_forall2; split => //=. move => x y HIn.
+			apply Forall2_forall2 in H15; destruct H15. apply H14 in HIn. inversion HIn; destruct H15 as [? [? ?]].
+			eapply Function_instance_ok__ with (v_C := v_C); repeat split => //=.
+			eapply module_inst_typing_extension; eauto.
+		- apply Forall2_forall2; split => //=. move => x y HIn.
+			apply Forall2_forall2 in H16; destruct H16. apply H14 in HIn. inversion HIn. destruct H16 as [? [? ?]].
+			eapply Global_instance_ok__; repeat split; eauto.
+		- apply Forall2_forall2; split => //=. move => x y HIn.
+			apply Forall2_forall2 in H17; destruct H17. apply H14 in HIn. inversion HIn; decomp; subst.
+			inversion H25. inversion H19; subst; destruct H27.
+			eapply Table_instance_ok__; repeat split; eauto.
+			apply Forall2_forall2; split => //=; move => x' y' HIn'. 
+			apply Forall2_forall2 in H24; destruct H24.
+			apply H24 in HIn'. 
+			apply Forall2_forall2 in HIn'; destruct HIn'.
+			apply Forall2_forall2; split => //=; move => x'' y'' HIn''.
+			apply H27 in HIn''. 
+			inversion HIn''; decomp; subst.
+			eapply Externaddrs_ok__func; eauto.
+		- eapply Forall2_list_update_func; eauto.
+			- apply Forall2_forall2; split => //=; move => x y HIn.
+				apply Forall2_forall2 in H18. apply H18 in HIn.
+				inversion HIn; decomp; subst.
+				eapply Memory_instance_ok__; eauto.
+			- 	
+				inversion H1; decomp; subst. simpl in *.
+				removeinstSimpler H27.
+				removeinstSimpler H28.
+				removeinstSimpler H30.
+				rewrite H7 in H21.
+				removeinstSimpler H29.
+				subst.
+				simpl in *.
+				apply Forall2_lookup in H33; destruct H33.
+				inversion HIT; decomp; subst; simpl in *.
+				apply Forall2_lookup2 in H37; destruct H37.
+				apply H26 in H0. inversion H0. destruct H41 as [? [? ?]]; simpl in H41.
+				simpl in H42. 
+				apply H19 in H41 as H'.
+				rewrite H42 in H'.
+				inversion H'. subst.
+				unfold set.
+				rewrite H42. simpl.
+				apply Forall2_lookup in H18; destruct H18.
+				apply H37 in H41.
+				inversion H41; decomp; subst.
+				rewrite H42 in H39.
+				injection H39 as ?.
+				rewrite H39.
+				rewrite H39 in H48.
+				inversion H48. inversion H46; decomp.
+				eapply Memory_instance_ok__; repeat split; eauto.
+	- (* Store Pack Val *)
+		destruct H3; destruct H1; subst.
+		apply_composition_typing_and_single HType.
+		apply_composition_typing_and_single H4_comp.
+		apply AI_const_typing in H4_comp0.
+		apply AI_const_typing in H4_comp.
+		rewrite <- admin_instrs_ok_eq in H4_comp1.
+		apply Store_typing in H4_comp1; destruct H4_comp1 as [v_n' [v_mt' [v_inn' [? [? [? [? [? ?]]]]]]]].
+		subst.
+		remember (s <| MEMS :=
+		list_update_func (MEMS s)
+		  (lookup_total (MODULE_MEMS (F_MODULE f)) 0)
+		  (λ v_1 : meminst,
+			 v_1 <| BYTES :=
+			 list_slice_update (BYTES v_1)
+			   (v_i + OFFSET v_mo)%coq_nat (v_n / 8)
+			   (fun_ibytes v_n
+				  (fun_wrap (fun_size (valtype__INN v_inn)) v_n v_c)) |>) |>) as s'.
+		assert (Store_extension s s').
+		{
+			eapply Store_extension__ with (v_meminst_1 := (MEMS s)) (v_meminst_1' := (MEMS s')) (v_meminst_2 := []);
+			repeat split; subst; simpl; try rewrite <- app_right_nil => //=.
+			- by rewrite list_update_length_func.
+			- by eapply func_extension_same.
+			- by eapply table_extension_same.
+			- (* Mem extension *)
+				inversion HIT; decomp; subst; simpl in *.
+				apply Forall2_lookup2 in H15; destruct H15. apply H7 in H0.
+				inversion H0; decomp; subst.
+				inversion HStore; decomp; subst; simpl in *.
+				eapply Forall2_list_update_func2; eauto.
+				- by apply mem_extension_same.
+				- unfold set; simpl. destruct v_mt'. apply mk_Mem_extension => //=.
+			- inversion HStore; decomp; subst; simpl in *.
+				eapply global_extension_same; eauto.
+		}
+		split => //=.
+		eapply update_mem_unchagned_func in Heqs' as ?; decomp.
+		subst; simpl in *.
+		destruct s. simpl in *.
+		inversion HStore; decomp; subst. 
+		injection H14 as ?; subst.
+		eapply Store_ok__OK; repeat split; simpl; eauto.
+		- erewrite list_update_length_func; eauto.
+		- apply Forall2_forall2; split => //=. move => x y HIn.
+			apply Forall2_forall2 in H15; destruct H15. apply H14 in HIn. inversion HIn; destruct H15 as [? [? ?]].
+			eapply Function_instance_ok__ with (v_C := v_C); repeat split => //=.
+			eapply module_inst_typing_extension; eauto.
+		- apply Forall2_forall2; split => //=. move => x y HIn.
+			apply Forall2_forall2 in H16; destruct H16. apply H14 in HIn. inversion HIn. destruct H16 as [? [? ?]].
+			eapply Global_instance_ok__; repeat split; eauto.
+		- apply Forall2_forall2; split => //=. move => x y HIn.
+			apply Forall2_forall2 in H17; destruct H17. apply H14 in HIn. inversion HIn; decomp; subst.
+			inversion H25. inversion H19; subst. destruct H27.
+			eapply Table_instance_ok__; repeat split; eauto.
+			apply Forall2_forall2; split => //=; move => x' y' HIn'. 
+			apply Forall2_forall2 in H24; destruct H24.
+			apply H24 in HIn'. 
+			apply Forall2_forall2 in HIn'; destruct HIn'.
+			apply Forall2_forall2; split => //=; move => x'' y'' HIn''.
+			apply H27 in HIn''. 
+			inversion HIn''; decomp; subst.
+			eapply Externaddrs_ok__func; eauto.
+		- eapply Forall2_list_update_func; eauto.
+			- apply Forall2_forall2; split => //=; move => x y HIn.
+				apply Forall2_forall2 in H18. apply H18 in HIn.
+				inversion HIn; decomp; subst.
+				eapply Memory_instance_ok__; eauto.
+			- 	
+				inversion H1; decomp; subst. simpl in *.
+				removeinstSimpler H27.
+				removeinstSimpler H28.
+				removeinstSimpler H30.
+				rewrite H7 in H21.
+				removeinstSimpler H29.
+				subst.
+				simpl in *.
+				apply Forall2_lookup in H33; destruct H33.
+				inversion HIT; decomp; subst; simpl in *.
+				apply Forall2_lookup2 in H37; destruct H37.
+				apply H26 in H0. inversion H0. destruct H41 as [? [? ?]]; simpl in H41.
+				simpl in H42. 
+				apply H19 in H41 as H'.
+				rewrite H42 in H'.
+				inversion H'. subst.
+				unfold set.
+				rewrite H42. simpl.
+				apply Forall2_lookup in H18; destruct H18.
+				apply H37 in H41.
+				inversion H41; decomp; subst.
+				rewrite H42 in H39.
+				injection H39 as ?.
+				rewrite H39.
+				rewrite H39 in H48.
+				inversion H48. inversion H46; decomp.
+				eapply Memory_instance_ok__; repeat split; eauto.
+	- (* Memory Grow Succeed *)
+		destruct H3; destruct H1; subst.
+		apply_composition_typing_and_single HType.
+		rewrite <- admin_instrs_ok_eq in H4_comp.
+		apply Grow_memory_typing in H4_comp; destruct H4_comp as [v_mt' [ts' [? [? [? ?]]]]].
+		subst.
+		remember (s <| MEMS :=
+		list_update (MEMS s)
+		  (lookup_total (MODULE_MEMS (F_MODULE f)) 0) v_mi |>) as s'.
+
+		assert (Store_extension s s').
+		{
+			eapply Store_extension__ with (v_meminst_1 := (MEMS s)) (v_meminst_1' := (MEMS s')) (v_meminst_2 := []);
+			repeat split; subst s'; simpl; try rewrite <- app_right_nil => //=.
+			- by rewrite list_update_length.
+			- by eapply func_extension_same.
+			- by eapply table_extension_same.
+			- (* Mem extension *)
+				inversion HIT; decomp; subst; simpl in *.
+				apply Forall2_lookup2 in H13; destruct H13. apply H5 in H0.
+				inversion H0; decomp; subst.
+				inversion HStore; decomp; subst; simpl in *.
+				eapply Forall2_list_update2; eauto.
+				- by apply mem_extension_same.
+				- unfold fun_mem in H.
+					inversion H; decomp; subst.
+					simpl in H15. rewrite <- H1 in H15. simpl in H15. rewrite H15 in H18.
+					injection H18 as ?; subst.
+					apply mk_Mem_extension => //=.
+					apply leadd.
+			- inversion HStore; decomp; subst; simpl in *.
+				eapply global_extension_same; eauto.
+		}
+		split => //=.
+		eapply update_mem_unchagned in Heqs' as ?; decomp.
+		subst; simpl in *.
+		destruct s. simpl in *.
+		inversion HStore; decomp; subst. 
+		injection H12 as ?; subst.
+		inversion H; decomp.
+		unfold fun_mem in H8.
+
+		eapply Store_ok__OK with (v_memtype := list_update v_memtype ((lookup_total (MODULE_MEMS (F_MODULE f)) 0)) (limits__ (v_i + v_n)%coq_nat v_j)); repeat split; simpl; eauto.
+		- erewrite list_update_length; rewrite list_update_length; eauto.
+		- apply Forall2_forall2; split => //=. move => x y HIn.
+			apply Forall2_forall2 in H13; destruct H13. apply H22 in HIn. inversion HIn. destruct H23 as [? [? ?]].
+			eapply Function_instance_ok__ with (v_C := v_C); repeat split => //=.
+			eapply module_inst_typing_extension; eauto.
+		- apply Forall2_forall2; split => //=. move => x y HIn.
+			apply Forall2_forall2 in H14; destruct H14. apply H22 in HIn. inversion HIn. destruct H23 as [? [? ?]].
+			eapply Global_instance_ok__; repeat split; eauto.
+		- apply Forall2_forall2; split => //=. move => x y HIn.
+			apply Forall2_forall2 in H15; destruct H15. apply H22 in HIn. inversion HIn; decomp; subst.
+			inversion H30. inversion H12; subst. destruct H24.
+			eapply Table_instance_ok__; repeat split; eauto.
+			apply Forall2_forall2; split => //=; move => x' y' HIn'. 
+			apply Forall2_forall2 in H29; destruct H29.
+			apply H20 in HIn'. 
+			apply Forall2_forall2 in HIn'; destruct HIn'.
+			apply Forall2_forall2; split => //=; move => x'' y'' HIn''.
+			apply H25 in HIn''. 
+			inversion HIn''; decomp; subst.
+			eapply Externaddrs_ok__func; eauto.
+		- 	
+			eapply Forall2_list_update_both; eauto.
+			- apply Forall2_forall2; split => //=; move => x y HIn.
+				apply Forall2_forall2 in H16; destruct H16. apply H22 in HIn.
+				inversion HIn; decomp; subst.
+				eapply Memory_instance_ok__; eauto.
+			-
+				subst.
+				eapply Memory_instance_ok__; split; eauto.
+				eapply Memtype_ok__OK.
+				eapply Limits_ok__; split; eauto.
+				simpl in H8.
+				inversion HIT; decomp; subst.
+				rewrite <- H12 in H8.
+				simpl in H8.
+				apply Forall2_lookup in H16; destruct H16.
+				simpl in H0.
+				apply Forall2_lookup2 in H28; destruct H28.
+				apply H28 in H0. inversion H0; decomp.
+				simpl in H33.
+				apply H17 in H33.
+				rewrite H8 in H33.
+				inversion H33.
+				destruct H38.
+				inversion H41.
+				inversion H42.
+				decomp.
+				apply H48.
+Qed. *)
+	
+Lemma reduce_inst_unchanged: forall s f ais s' f' ais',
+    Step (mk_config (mk_state s f) ais) (mk_config (mk_state s' f') ais') ->
+    F_MODULE f = F_MODULE f'.
+Admitted.
+(* Proof.
+	move => s f ais s' f' ais' HReduce.
+	remember (mk_config (mk_state s f) ais) as c1.
+	remember (mk_config (mk_state s' f') ais') as c2.
+	generalize dependent ais. generalize dependent ais'.
+	induction HReduce; try intros; try (induction v_z); try induction v_z'; try (apply config_same in Heqc1;
+	apply config_same in Heqc2; destruct Heqc1 as [? [? ?]];
+	destruct Heqc2 as [? [? ?]]; subst => //).
+	eapply IHHReduce; eauto.
+Qed. *)
+
+Theorem t_pure_preservation: forall v_s v_minst v_ais v_ais' v_C loc lab ret tf,
+    Module_instance_ok v_s v_minst v_C ->
+    Admin_instrs_ok v_s (upd_label (upd_local_return v_C loc ret) lab) v_ais tf ->
+    Step_pure v_ais v_ais' ->
+    Admin_instrs_ok v_s (upd_label (upd_local_return v_C loc ret) lab) v_ais' tf.
+Proof.
+	move => v_s v_minst v_ais v_ais' v_C loc lab ret tf HInstType HType HReduce.
+	inversion HReduce; subst.
+	- eapply Step_pure__unreachable_preserves; eauto.
+	- eapply Step_pure__nop_preserves; eauto.
+	- eapply Step_pure__drop_preserves; eauto.
+	- eapply Step_pure__select_true_preserves; eauto.
+	- eapply Step_pure__select_false_preserves; eauto.
+	- eapply Step_pure__if_true_preserves; eauto.
+	- eapply Step_pure__if_false_preserves; eauto.
+	- eapply Step_pure__label_vals_preserves; eauto.
+Admitted. (*
+	- eapply Step_pure__br_zero_preserves; eauto.
+	- eapply Step_pure__br_succ_preserves; eauto.
+	- eapply Step_pure__br_if_true_preserves; eauto.
+	- eapply Step_pure__br_if_false_preserves; eauto.
+	- eapply Step_pure__br_table_lt_preserves; eauto.
+	- eapply Step_pure__br_table_ge_preserves; eauto.
+	- eapply Step_pure__frame_vals_preserves; eauto.
+	- eapply Step_pure__return_frame_preserves; eauto.
+	- eapply Step_pure__return_label_preserves; eauto.
+	- eapply Step_pure__trap_vals_preserves; eauto.
+	- eapply Step_pure__trap_label_preserves; eauto.
+	- eapply Step_pure__trap_frame_preserves; eauto.
+	- eapply Step_pure__unop_val_preserves; eauto.
+	- eapply Step_pure__unop_trap_preserves; eauto.
+	- eapply Step_pure__binop_val_preserves; eauto.
+	- eapply Step_pure__binop_trap_preserves; eauto.
+	- eapply Step_pure__testop_preserves; eauto.
+	- eapply Step_pure__relop_preserves; eauto.
+	- eapply Step_pure__cvtop_val_preserves; eauto.
+	- eapply Step_pure__cvtop_trap_preserves; eauto.
+	- eapply Step_pure__local_tee_preserves; eauto.
+Qed. *)
+
+Lemma t_read_preservation: forall v_s v_f v_ais v_ais' v_C v_t1 t1s t2s lab ret,
+    Step_read (mk_config (mk_state v_s v_f) v_ais) v_ais' ->
+    Store_ok v_s ->
+    Module_instance_ok v_s (F_MODULE v_f) v_C ->
+	Forall2 (fun v_t v_val => Val_ok v_val v_t) v_t1 (LOCALS v_f) ->
+    Admin_instrs_ok v_s (upd_label (upd_local_return v_C (v_t1 ++ C_LOCALS v_C) ret) lab) v_ais (mk_functype t1s t2s) ->
+    Admin_instrs_ok v_s (upd_label (upd_local_return v_C (v_t1 ++ C_LOCALS v_C) ret) lab) v_ais' (mk_functype t1s t2s).
+Proof.
+	move => v_s v_f v_ais v_ais' v_C v_t1 t1s t2s lab ret HReduce HST.
+	move: v_C ret lab t1s t2s.
+	remember (mk_config (mk_state v_s v_f) v_ais) as c1.
+	induction HReduce; move => C ret lab tx ty HIT1 HValOK HType; decomp; destruct v_z; try eauto;
+	try (apply config_same in Heqc1; destruct Heqc1 as [Hbefore1 [Hbefore2 Hbefore3]]; subst => //).
+	- eapply Step_read__block_preserves; eauto.
+	- Admitted. (* eapply Step_read__loop_preserves; eauto.
+	- eapply Step_read__call_preserves; eauto.
+	- eapply Step_read__call_indirect_call_preserves; eauto.
+	- eapply Step_read__call_indirect_trap_preserves; eauto.
+	- eapply Step_read__call_addr_preserves; eauto.
+	- eapply Step_read__local_get_preserves; eauto.
+	- eapply Step_read__global_get_preserves; eauto.
+	- eapply Step_read__load_num_trap_preserves; eauto.
+	- eapply Step_read__load_num_val_preserves; eauto.
+	- eapply Step_read__load_pack_trap_preserves; eauto.
+	- eapply Step_read__load_pack_val_preserves; eauto.
+	- eapply Step_read__memory_size_preserves; eauto.
+Qed. *)
+
+Lemma t_preservation_type: forall v_s v_f v_ais v_s' v_f' v_ais' v_C v_t1 t1s t2s lab ret,
+    Step (mk_config (mk_state v_s v_f) v_ais) (mk_config (mk_state v_s' v_f') v_ais') ->
+    Store_ok v_s ->
+    Store_ok v_s' ->
+	Store_extension v_s v_s' -> 
+    Module_instance_ok v_s (F_MODULE v_f) v_C ->
+    Module_instance_ok v_s' (F_MODULE v_f) v_C ->
+	Forall2 (fun v_t v_val => Val_ok v_val v_t) v_t1 (LOCALS v_f) ->
+    Admin_instrs_ok v_s (upd_label (upd_local_return v_C (v_t1 ++ C_LOCALS v_C) ret) lab) v_ais (mk_functype t1s t2s) ->
+    Admin_instrs_ok v_s' (upd_label (upd_local_return v_C (v_t1 ++ C_LOCALS v_C) ret) lab) v_ais' (mk_functype t1s t2s).
+Admitted.
+(* Proof.
+	move => v_s v_f v_ais v_s' v_f' v_ais' v_C v_t1 t1s t2s lab ret HReduce HST1 HST2 HSExt.
+	move: v_C ret lab t1s t2s.
+	remember (mk_config (mk_state v_s v_f) v_ais) as c1.
+	remember (mk_config (mk_state v_s' v_f') v_ais') as c2.
+	generalize dependent v_ais.
+	generalize dependent v_ais'.
+	generalize dependent v_t1.
+	generalize dependent v_f.
+	generalize dependent v_f'.
+	induction HReduce; move => r_v_f' r_v_f v_t1 v_ais' Heqc2 v_ais Heqc1 v_C ret lab tx ty HIT1 HIT2 HValOK HType; try (destruct v_z; subst);  try (destruct v_z'; subst); try eauto;
+	try (apply config_same in Heqc1; apply config_same in Heqc2; 
+		destruct Heqc1 as [Hbefore1 [Hbefore2 Hbefore3]]; 
+		destruct Heqc2 as [Hafter1 [Hafter2 Hafter3]]; subst => //).
+	- (* Step_pure *) eapply t_pure_preservation; eauto.
+	- (* Step_read *) eapply t_read_preservation; eauto.
+	- (* Context Label *) 
+		rewrite <- admin_instrs_ok_eq in HType.
+		apply Label_typing in HType as H. destruct H as [ts [ts2' [? [? [? ?]]]]].
+		subst.
+		apply admin_instrs_weakening_empty_1.
+		rewrite <- admin_instrs_ok_eq.
+		apply AI_ok_label with (v_t_1 := ts).
+		repeat split => //=.
+		eapply IHHReduce => //=.
+	- (* Context Frame *)
+		rewrite <- admin_instrs_ok_eq in HType.
+		apply Frame_typing in HType as H. destruct H as [ts [? [? ?]]].
+		subst.
+		apply admin_instrs_weakening_empty_1.
+		rewrite <- admin_instrs_ok_eq.
+		apply AI_ok_frame.
+		split => //.
+		inversion H0. subst. destruct H.
+		apply Thread_ok__ with (v_C := v_C0).
+		inversion H; destruct H2 as [? [? ?]]. 
+		split.
+		- apply Frame_ok__.
+			repeat split => //=.
+			eapply module_inst_typing_extension; eauto.
+		-
+			apply inst_t_context_local_empty in H6 as H'.
+			rewrite upd_label_unchanged_typing.
+			remember v_t as val.
+			rewrite -> app_right_nil in Heqval.
+			rewrite <- H' in Heqval. subst.
+			eapply IHHReduce => //=.
+			eapply module_inst_typing_extension; eauto.
+	- (* Local set *)
+		apply_composition_typing_and_single HType.
+		destruct v_val.
+		apply AI_const_typing in H4_comp0.
+		rewrite <- admin_instrs_ok_eq in H4_comp.
+		apply Set_local_typing in H4_comp; destruct H4_comp as [t [? [? ?]]].
+		subst.
+		repeat rewrite -> app_assoc in H0; apply split_append_last in H0; destruct H0.
+		subst.
+		apply admin_weakening_empty_both.
+		apply AIs_ok_empty.
+	- (* Global set *)
+		apply_composition_typing_and_single HType.
+		destruct v_val.
+		apply AI_const_typing in H4_comp0.
+		rewrite <- admin_instrs_ok_eq in H4_comp.
+		apply Set_global_typing in H4_comp. destruct H4_comp as [t [? [? ?]]].
+		subst.
+		repeat rewrite -> app_assoc in H0; apply split_append_last in H0; destruct H0.
+		subst.
+		apply admin_weakening_empty_both.
+		apply AIs_ok_empty.
+	- (* Store Num Trap *)
+		rewrite <- admin_instrs_ok_eq.
+		apply AI_ok_trap.
+	- (* Store Num Val *)
+		apply_composition_typing HType.
+		apply_composition_typing_and_single H4_comp.
+		rewrite <- admin_instrs_ok_eq in H3_comp.
+		apply AI_const_typing in H3_comp.
+		apply AI_const_typing in H4_comp.
+		rewrite <- admin_instrs_ok_eq in H4_comp0.
+		apply Store_typing in H4_comp0; destruct H4_comp0 as [v_n [v_mt [v_inn [? [? [? [? [? ?]]]]]]]].
+		subst.
+		remember [:: I32; v_t] as v_t'.
+		rewrite -cat1s in Heqv_t'.
+		subst.
+		repeat rewrite -> app_assoc in H; apply split_append_last in H; destruct H; subst.
+		rewrite H in H1_comp0.
+		repeat rewrite -> app_assoc in H1_comp0; apply split_append_last in H1_comp0; destruct H1_comp0; subst.
+		subst.
+		apply admin_weakening_empty_both.
+		apply AIs_ok_empty.
+	- (* Store Pack Trap *)
+		rewrite <- admin_instrs_ok_eq.
+		apply AI_ok_trap.
+	- (* Store Pack Val *)
+		apply_composition_typing HType.
+		apply_composition_typing_and_single H4_comp.
+		rewrite <- admin_instrs_ok_eq in H3_comp.
+		apply AI_const_typing in H3_comp.
+		apply AI_const_typing in H4_comp.
+		rewrite <- admin_instrs_ok_eq in H4_comp0.
+		apply Store_typing in H4_comp0; destruct H4_comp0 as [v_n' [v_mt' [v_inn' [? [? [? [? [? ?]]]]]]]].
+		subst.
+		remember [:: I32; valtype__INN v_inn] as v_t'.
+		rewrite -cat1s in Heqv_t'.
+		subst.
+		repeat rewrite -> app_assoc in H; apply split_append_last in H; destruct H; subst.
+		rewrite H in H1_comp0.
+		repeat rewrite -> app_assoc in H1_comp0; apply split_append_last in H1_comp0; destruct H1_comp0; subst.
+		subst.
+		apply admin_weakening_empty_both.
+		apply AIs_ok_empty.
+	- (* Memory Grow Succeed *)
+		apply_composition_typing_and_single HType.
+		apply AI_const_typing in H4_comp0.
+		rewrite <- admin_instrs_ok_eq in H4_comp.
+		apply Grow_memory_typing in H4_comp; destruct H4_comp as [v_mt [ts [? [? [? ?]]]]].
+		subst.
+		repeat rewrite -> app_assoc in H3; apply split_append_last in H3; destruct H3; subst.
+		repeat rewrite -> app_assoc.
+		apply admin_instrs_weakening_empty_1.
+		rewrite <- admin_instrs_ok_eq.
+		remember (Datatypes.length (BYTES (fun_mem (mk_state v_s r_v_f) 0)) / (64 * fun_Ki)%coq_nat) as v_n'.
+		eapply (AI_ok_instr _ _ (CONST (I32) v_n') (mk_functype [] [(I32)])).
+		apply const.
+	- (* Memory Grow Fail *)
+		apply_composition_typing_and_single HType.
+		apply AI_const_typing in H4_comp0.
+		rewrite <- admin_instrs_ok_eq in H4_comp.
+		apply Grow_memory_typing in H4_comp; destruct H4_comp as [v_mt [ts [? [? [? ?]]]]].
+		subst.
+		repeat rewrite -> app_assoc in H2; apply split_append_last in H2; destruct H2; subst.
+		repeat rewrite -> app_assoc.
+		apply admin_instrs_weakening_empty_1.
+		rewrite <- admin_instrs_ok_eq.
+		remember (fun_invsigned 32 (0 - 1)%coq_nat) as v_n'.
+		eapply (AI_ok_instr _ _ (CONST (I32) v_n') (mk_functype [] [(I32)])).
+		apply const.
+Qed. *)
+
+(* Ultimate goal of project *)				
 Theorem t_preservation: forall c1 ts c2,
 	Step c1 c2 ->
 	Config_ok c1 ts ->
 	Config_ok c2 ts.
-Proof.
-	move=> c1 ts c2 HStep HType.
 Admitted.
+(* Proof.
+	move => c1 ts c2 HReduce HType.
+	destruct c1; destruct v_state as [store1 frame1].
+	destruct c2; destruct v_state as [store2 frame2].
+	inversion HType; destruct H3.
+	inversion H4; destruct H5.
+	rewrite <- upd_return_is_same_as_append in H11.
+	inversion H5. destruct H12 as [H0' [H1' H2']].
+	rewrite <- upd_local_is_same_as_append in H15.
+	subst.
+	rewrite <- upd_local_return_is_same_as_append in H11.
+	apply upd_label_unchanged_typing in H11.
+	assert (Store_extension store1 store2 /\ Store_ok store2).
+	{
+		apply (store_extension_reduce 
+			store1  
+			{|LOCALS := v_val;F_MODULE := v_moduleinst|} 
+			v__ store2 frame2 v__0 v_C0 (mk_functype [::] ts) 
+			(_append v_t1 (C_LOCALS v_C0)) 
+			(C_LABELS (upd_local_return v_C0 (_append v_t1 (C_LOCALS v_C0)) (_append (option_map [eta Some] None) (C_RETURN v_C0))))
+			(_append (Some None) (C_RETURN v_C0))) => //.
+	}
+	destruct H.
+	apply reduce_inst_unchanged in HReduce as HModuleInst.
+	destruct frame2 as [locals2 module2].
+	simpl in HModuleInst.
+	remember {|LOCALS := v_val;F_MODULE := v_moduleinst|} as f.
+	assert (Module_instance_ok store2 v_moduleinst v_C0). { apply (module_inst_typing_extension store1); eauto. }
+	apply Config_ok__; split => //=.
+	eapply Thread_ok__; split => //=.
+	rewrite <- HModuleInst.
+	eapply (Frame_ok__ store2 locals2 v_moduleinst v_C0 v_t1); eauto.
+	apply (t_preservation_vs_type) with (v_t1 := v_t1) (C := v_C0) (C' := v_C0) 
+		(lab:= (C_LABELS (upd_local_return v_C0 (_append v_t1 (C_LOCALS v_C0)) (_append (option_map [eta Some] None) (C_RETURN v_C0))))) 
+		(ret:= (_append (Some None) (C_RETURN v_C0))) (t1s := []) (t2s := ts) in HReduce as H10; try destruct H10; try apply Forall2_length in H10; repeat split => //.
+	- apply H3.
+	- apply H0.
+	- by rewrite Heqf.
+	- by rewrite <- HModuleInst.
+	- simpl. apply inst_t_context_local_empty in H1. rewrite H1. by rewrite -> app_nil_r.
+	- by rewrite Heqf.
+	- apply H11.
+	(* Actual Typing proof *)
+	rewrite <- upd_return_is_same_as_append; simpl.
+	rewrite <- upd_local_is_same_as_append; simpl.
+	fold_upd_context.
+	rewrite -> _append_option_none_left.
+	rewrite upd_label_unchanged_typing.
+	eapply t_preservation_type; eauto; try rewrite -> Heqf; eauto.
+Qed. *)
